refactor(compiler) Reorganization and renaming for internal types
Signed-off-by: Jerome Simeon <jeromesimeon@me.com>

packages/ergo-cli/extracted/ergotopcore.js
@@ -28876,7 +28876,25 @@ b=a[2];if(!fn(au,a[1],b)){var
 a=b;continue}var
 d=0}else
 var
-d=1;return d?E(f,0):[1,l(e,Qj(c))]}},wB=function(a){return a[2]},qc=function(a){return 0===a[0]?[0,a[1]]:0},qd=function(a){return 0},Xw=function(a){return au(a,mF)?0:[0,[0,a,mF],0]},Xx=function(a){return au(a,kX)?0:[0,[0,a,kX],0]},Xy=function(a){return au(a,mG)?0:[0,[0,a,mG],0]},Xz=function(a){return au(a,mH)?0:[0,[0,a,mH],0]},iX=function(c,b,a){return a?[0,[0,b,a[1]],0]:l(c,b)},XA=function(a){return 12===a[0]?[0,a[2]]:0},wC=function(b,a){var
+d=1;return d?E(f,0):[1,l(e,Qj(c))]}},wB=function(a){return a[2]},qc=function(a){return 0===a[0]?[0,a[1]]:0},qd=function(a){return 0},Xw=function(a){return au(a,mF)?0:[0,[0,a,mF],0]},Xx=function(a){return au(a,kX)?0:[0,[0,a,kX],0]},Xy=function(a){return au(a,mG)?0:[0,[0,a,mG],0]},Xz=function(a){return au(a,mH)?0:[0,[0,a,mH],0]},iX=function(c,b,a){return a?[0,[0,b,a[1]],0]:l(c,b)},XA=function(a){return 12===a[0]?[0,a[2]]:0},kY=function(c){var
+a=r_(gs,c),e=aW(function(a){return[0,a[2],a]},a),b=aW(function(d){var
+c=d[3],b=d[2];switch(c[0]){case
+0:var
+a=iX(qd,b,0);break;case
+1:var
+a=iX(Xw,b,c[2]);break;case
+2:var
+a=iX(qd,b,c[2]);break;case
+3:var
+a=iX(Xx,b,c[2]);break;case
+4:var
+a=iX(Xy,b,c[2]);break;case
+5:var
+a=iX(Xz,b,c[2]);break;case
+8:var
+a=iX(qd,b,0);break;default:var
+a=0}return[0,d,h7(aW(function(b){var
+a=b7(au,e,b[2]);return a?[0,a[1],0]:0},a))]},a);return u_(wB,function(a){return cv(a[2])},b)},wC=function(b,a){var
 c=b6(b[4],a[4]),d=b6(b[3],a[3]),e=b6(b[2],a[2]);return[0,b6(b[1],a[1]),e,d,c]},wD=function(d,c,a){var
 b=b7(au,c[1],a);return b?E(b[1][1],0):[1,[2,d,s(Wv,s(a,Wu))]]},wE=function(b,e,a){var
 c=b7(au,e[2],a);if(c){var
@@ -28886,19 +28904,19 @@ d=b7(au,f[2],a);if(d){var
 e=d[1],b=e[2],g=e[1];if(typeof
 b!=="number"&&0===b[0])return E([0,g,b[1]],0);return qa(c,a)}return qa(c,a)},wG=function(d,c,a){var
 b=b7(au,c[3],a);return b?E(b[1][1],0):[1,[2,d,s(WD,s(a,WC))]]},wH=function(d,c,a){var
-b=b7(au,c[4],a);return b?E(b[1][1],0):[1,[2,d,s(WF,s(a,WE))]]},wI=function(d,c,b,a){return[0,[0,[0,d,[0,c,b]],a[1]],a[2],a[3],a[4]]},qe=function(d,c,b,a){return[0,a[1],[0,[0,d,[0,c,b]],a[2]],a[3],a[4]]},wJ=function(c,b,a){return[0,a[1],a[2],[0,[0,c,[0,b,0]],a[3]],a[4]]},wK=function(c,b,a){return[0,a[1],a[2],a[3],[0,[0,c,[0,b,0]],a[4]]]},XB=function(a){return[0,0,a,g0,g0,0]},kY=function(a,b,c){var
+b=b7(au,c[4],a);return b?E(b[1][1],0):[1,[2,d,s(WF,s(a,WE))]]},wI=function(d,c,b,a){return[0,[0,[0,d,[0,c,b]],a[1]],a[2],a[3],a[4]]},qe=function(d,c,b,a){return[0,a[1],[0,[0,d,[0,c,b]],a[2]],a[3],a[4]]},wJ=function(c,b,a){return[0,a[1],a[2],[0,[0,c,[0,b,0]],a[3]],a[4]]},wK=function(c,b,a){return[0,a[1],a[2],a[3],[0,[0,c,[0,b,0]],a[4]]]},XB=function(a){return[0,0,a,g0,g0,0]},kZ=function(a,b,c){var
 d=b7(au,a[1],b);if(d){var
 e=a[5],f=a[4],g=a[3],h=a[2],i=l(c,d[1]);return[0,mu(au,a[1],b,i),h,g,f,e]}var
 j=a[5],k=a[4],m=a[3],n=a[2],o=a[1];return[0,[0,[0,b,l(c,g0)],o],n,m,k,j]},jE=function(a,b){var
 c=a[5],d=l(b,a[4]),e=l(b,a[3]);return[0,a[1],a[2],e,d,c]},qf=function(a,f){return jE(a,function(a){var
 b=a[4],c=a[3],d=a[2],e=ht(function(a){return au(f,a[1])?0:1},d);return[0,a[1],e,c,b]})},qg=function(a,d){var
 b=a[2],f=a[3],c=a[1],e=a[5];if(au(b,wi))return[0,c,d,g0,g0,e];var
-g=b7(au,c,b);return g?[0,mu(au,c,b,wC(f,g[1])),d,g0,g0,e]:[0,[0,[0,b,f],c],d,g0,g0,e]},kZ=function(f,c,a,b,e){var
+g=b7(au,c,b);return g?[0,mu(au,c,b,wC(f,g[1])),d,g0,g0,e]:[0,[0,[0,b,f],c],d,g0,g0,e]},k0=function(f,c,a,b,e){var
 d=b7(au,[0,[0,a[2],a[4]],a[1]],b);return d?aG(f,c,d[1],e):[1,[2,c,s(Wx,s(b,Ww))]]},mI=function(c,b,a){var
-d=a[1],e=b[4];return d?kZ(wD,c,b,d[1],a[2]):wD(c,e,a[2])},wL=function(c,b,a){var
-d=a[1],e=b[4];return d?kZ(wF,c,b,d[1],a[2]):wF(c,e,a[2])},wM=function(c,b,a){var
-d=a[1],f=b[4],e=d?kZ(wE,c,b,d[1],a[2]):wE(c,f,a[2]);return 0===e[0]?e:B(dJ,wL(c,b,a))},wN=function(c,b,a){var
-d=a[1],e=b[4];return d?kZ(wH,c,b,d[1],a[2]):wH(c,e,a[2])},jF=function(a){switch(a[0]){case
+d=a[1],e=b[4];return d?k0(wD,c,b,d[1],a[2]):wD(c,e,a[2])},wL=function(c,b,a){var
+d=a[1],e=b[4];return d?k0(wF,c,b,d[1],a[2]):wF(c,e,a[2])},wM=function(c,b,a){var
+d=a[1],f=b[4],e=d?k0(wE,c,b,d[1],a[2]):wE(c,f,a[2]);return 0===e[0]?e:B(dJ,wL(c,b,a))},wN=function(c,b,a){var
+d=a[1],e=b[4];return d?k0(wH,c,b,d[1],a[2]):wH(c,e,a[2])},jF=function(a){switch(a[0]){case
 0:return a[1];case
 1:return a[1];case
 2:return a[1];case
@@ -28968,7 +28986,7 @@ W=V[2],az=V[1],e=function(a){return 0!==(az&1<<a)?1:0},a7=e(7),a8=e(6),a9=e(5),a
 X=W[2],aA=W[1],d=function(a){return 0!==(aA&1<<a)?1:0},a0=d(7),a1=d(6),a2=d(5),a3=d(4),a4=d(3),a5=d(2),a6=d(1);if(d(0))return 0;if(a6)return 0;if(a5){if(a4)return 0;if(a3){if(a2){if(a1){if(a0)return 0;if(X){var
 Y=X[2],aB=X[1],c=function(a){return 0!==(aB&1<<a)?1:0},aT=c(7),aU=c(6),aV=c(5),aW=c(4),aX=c(3),aY=c(2),aZ=c(1);if(c(0)){if(aZ)return 0;if(aY)return 0;if(aX)return 0;if(aW)return 0;if(aV){if(aU){if(aT)return 0;if(Y){var
 Z=Y[2],aC=Y[1],b=function(a){return 0!==(aC&1<<a)?1:0},aM=b(7),aN=b(6),aO=b(5),aP=b(4),aQ=b(3),aR=b(2),aS=b(1);if(b(0))return 0;if(aS)return 0;if(aR){if(aQ)return 0;if(aP){if(aO){if(aN){if(aM)return 0;if(Z){var
-aD=Z[2],aE=Z[1],a=function(a){return 0!==(aE&1<<a)?1:0},aF=a(7),aG=a(6),aH=a(5),aI=a(4),aJ=a(3),aK=a(2),aL=a(1);return a(0)?aL?0:aK?aJ?0:aI?0:aH?aG?aF?0:aD?0:av?0:[0,[0,[0,aj,ai],aw]]:0:0:0:0}return 0}return 0}return 0}return 0}return 0}return 0}return 0}return 0}return 0}return 0}return 0}return 0}return 0}return 0}return 0}return 0}return 0}return 0}return 0}return 0}return 0}return 0}return 0}return 0}return 0}return 0}return 0}return 0}return 0}return 0}return 0}return 0}return 0}return 0}return 0}return 0}return 0}return 0}return 0}return 0}return 0}return 0}return 0}return 0}return 0}return 0}return 0}return 0}return 0}return 0}return 0}return 0}return 0}return 0}return 0}return 0}return 0}return 0}return 0}return 0}return 0}return 0}return 0}return 0}return 0}return 0}return 0}return 0}return 0}return 0}return 0}return 0}return 0}return 0}return 0}return 0}return 0}return 0}return 0}return 0}return 0}return 0}return 0}return 0}return 0}return 0}return 0}return 0}return 0}return 0}return 0}return 0}return 0}return 0}return 0}return 0}return 0}return 0}return 0}return 0}return 0}return 0}return 0}return 0}return 0}return 0}return 0}return 0}return 0}return 0}return 0}return 0}return 0}return 0}return 0}return 0}return 0}return 0}return 0}return 0}return 0}return 0}return 0}return 0}return 0}return 0}return 0}return 0}return 0}return 0}return 0}return 0}return 0}return 0},XO=0,XP=2,k0=[0,vs(2*function(a){return 1+(2*a|0)|0}(XP)|0),XO],wR=function(d,c){var
+aD=Z[2],aE=Z[1],a=function(a){return 0!==(aE&1<<a)?1:0},aF=a(7),aG=a(6),aH=a(5),aI=a(4),aJ=a(3),aK=a(2),aL=a(1);return a(0)?aL?0:aK?aJ?0:aI?0:aH?aG?aF?0:aD?0:av?0:[0,[0,[0,aj,ai],aw]]:0:0:0:0}return 0}return 0}return 0}return 0}return 0}return 0}return 0}return 0}return 0}return 0}return 0}return 0}return 0}return 0}return 0}return 0}return 0}return 0}return 0}return 0}return 0}return 0}return 0}return 0}return 0}return 0}return 0}return 0}return 0}return 0}return 0}return 0}return 0}return 0}return 0}return 0}return 0}return 0}return 0}return 0}return 0}return 0}return 0}return 0}return 0}return 0}return 0}return 0}return 0}return 0}return 0}return 0}return 0}return 0}return 0}return 0}return 0}return 0}return 0}return 0}return 0}return 0}return 0}return 0}return 0}return 0}return 0}return 0}return 0}return 0}return 0}return 0}return 0}return 0}return 0}return 0}return 0}return 0}return 0}return 0}return 0}return 0}return 0}return 0}return 0}return 0}return 0}return 0}return 0}return 0}return 0}return 0}return 0}return 0}return 0}return 0}return 0}return 0}return 0}return 0}return 0}return 0}return 0}return 0}return 0}return 0}return 0}return 0}return 0}return 0}return 0}return 0}return 0}return 0}return 0}return 0}return 0}return 0}return 0}return 0}return 0}return 0}return 0}return 0}return 0}return 0}return 0}return 0}return 0}return 0}return 0}return 0}return 0}return 0},XO=0,XP=2,k1=[0,vs(2*function(a){return 1+(2*a|0)|0}(XP)|0),XO],wR=function(d,c){var
 a=c;for(;;){if(typeof
 a!=="number")switch(a[0]){case
 >>>>>>> Somewhat properly hooks up new JavaScript backend
@@ -29307,19 +29325,62 @@ i=c[1];return c[2]?wQ(b,c):qi(b,i)}return wQ(b,c);default:switch(a[1]){case
 3:return Yw;case
 4:return Yx;case
 5:return Yy;case
-6:return Yz;default:return Yv}}},aX=function(c,b,a){return jG(b,x(ah[36],c[1],a))},jH=function(c,b,a){return a?s(YA,aX(c,b,a[1])):0},k1=function(d,c,b,a){var
+6:return Yz;default:return Yv}}},aX=function(c,b,a){return jG(b,x(ah[36],c[1],a))},jH=function(c,b,a){return a?s(YA,aX(c,b,a[1])):0},k2=function(d,c,b,a){var
 e=s(YC,s(b,YB));return[0,ca,s(YD,s(jH(d,c,[0,a]),e))]},wS=function(b,c,a){var
-d=x(ah[25],b,a),e=k1(b,c,YE,a);return fq(av(h6,d),e,0)},f5=function(a,c,b,e){var
-f=x(ah[25],a,b),g=k1(a,c,YF,b),d=fq(av(dJ,f),g,0),h=B(dJ,aQ(function(d){var
-e=k1(a,c,mE,b);return fq(aG(ah[29],a,[1,mE],d),e,0)},d)),i=B(dJ,aQ(function(d){var
-e=k1(a,c,hw,b);return fq(aG(ah[29],a,[1,hw],d),e,0)},d)),j=B(dJ,aQ(function(d){var
-f=k1(a,c,fI,b);return fq(aG(ah[29],a,[1,fI],d),f,e)},d));return eP(function(c,b,a){return[0,[0,c,b],a]},h,i,j)},wT=function(c,b,a,d){var
+d=x(ah[25],b,a),e=k2(b,c,YE,a);return fq(av(h6,d),e,0)},f5=function(a,c,b,e){var
+f=x(ah[25],a,b),g=k2(a,c,YF,b),d=fq(av(dJ,f),g,0),h=B(dJ,aQ(function(d){var
+e=k2(a,c,mE,b);return fq(aG(ah[29],a,[1,mE],d),e,0)},d)),i=B(dJ,aQ(function(d){var
+e=k2(a,c,hw,b);return fq(aG(ah[29],a,[1,hw],d),e,0)},d)),j=B(dJ,aQ(function(d){var
+f=k2(a,c,fI,b);return fq(aG(ah[29],a,[1,fI],d),f,e)},d));return eP(function(c,b,a){return[0,[0,c,b],a]},h,i,j)},wT=function(c,b,a,d){var
 e=wS(c,b,a),f=f5(c,b,a,d);return aS(function(b,a){return[0,b,a]},f,e)},g1=function(d,a,c,b){var
 e=jH(d,a,b);return s(YG,s(eF(a,c),e))},g2=function(d,b,a,c){if(a){var
-e=a[2],f=a[1],g=s(jH(d,b,c),k0),h=aW(function(a){return eF(b,a)},e),i=s(YH,eF(b,f));return s(cF(function(b,a){return s(a,s(k0,s(YI,b)))},i,h),g)}return 0},g3=function(e,b,d,a,c){function
+e=a[2],f=a[1],g=s(jH(d,b,c),k1),h=aW(function(a){return eF(b,a)},e),i=s(YH,eF(b,f));return s(cF(function(b,a){return s(a,s(k1,s(YI,b)))},i,h),g)}return 0},g3=function(e,b,d,a,c){function
 f(a){return eF(b,a)}if(d){if(f3(a0,a,d[1]))return 0;var
-g=jH(e,b,c);return s(k0,s(YJ,s(f(a),g)))}var
-h=jH(e,b,c);return s(k0,s(YK,s(f(a),h)))},wU=function(i){var
+g=jH(e,b,c);return s(k1,s(YJ,s(f(a),g)))}var
+h=jH(e,b,c);return s(k1,s(YK,s(f(a),h)))},hx=function(a,g,b,f){var
+c=b7(au,a,b);if(c){var
+d=c[1],e=d[2],h=d[1];return 0===e[0]?[0,[0,g,[0,[0,b,h],[0,b6(e[1],f)]]],a]:a}return a},g4=function(a,b){switch(b[0]){case
+0:return l(ah[5],a);case
+1:return l(ah[4],a);case
+2:return l(ah[6],a);case
+3:return l(ah[9],a);case
+4:return l(ah[10],a);case
+5:return l(ah[7],a);case
+8:return l(ah[11],a);case
+9:return l(ah[12],a);case
+10:return l(ah[13],a);case
+11:return l(ah[14],a);case
+12:return x(ah[19],a,[0,b[2],0]);case
+13:var
+c=b[2],d=l(ah[6],a),e=g4(a,c);return aG(ah[17],a,e,d);case
+14:var
+f=b[2],g=aW(function(b){var
+c=g4(a,b[2]);return[0,b[1],c]},f),h=l(iO(f2),g);return aG(ah[16],a,ah[2],h);case
+15:var
+i=g4(a,b[2]);return x(ah[15],a,i);case
+16:var
+j=b[2],k=g4(a,b[3]),m=g4(a,j);return aG(ah[17],a,m,k);default:return l(ah[8],a)}},wU=function(a,b){if(b){var
+c=wU(a,b[2]),d=l(ah[10],a);return aG(ah[17],a,d,c)}return l(ah[10],a)},wV=function(f){var
+a=kY(f),c=0,b=em(function(b,n){var
+c=n[3],a=n[2];switch(c[0]){case
+0:return[0,[0,a,[0,[0,wg,0],[1,c[1]]]],b];case
+1:var
+d=c[3],h=c[2];return h?hx(b,a,h[1],d):au(a,mF)?[0,[0,a,[0,0,[0,d]]],b]:hx(b,a,mF,d);case
+2:var
+i=c[3],j=c[2];return j?hx(b,a,j[1],i):[0,[0,a,[0,0,[0,i]]],b];case
+3:var
+e=c[3],k=c[2];return k?hx(b,a,k[1],e):au(a,kX)?[0,[0,a,[0,0,[0,e]]],b]:hx(b,a,kX,e);case
+4:var
+f=c[3],l=c[2];return l?hx(b,a,l[1],f):au(a,mG)?[0,[0,a,[0,0,[0,f]]],b]:hx(b,a,mG,f);case
+5:var
+g=c[3],m=c[2];return m?hx(b,a,m[1],g):au(a,mH)?[0,[0,a,[0,0,[0,g]]],b]:hx(b,a,mH,g);default:return b}},a,c),d=h7(aW(function(a){var
+b=a[1],c=a[2][1];return aW(function(a){return[0,b,a]},c)},b)),e=wk(ca,l(ah[32],d)),g=aQ(function(a){var
+c=aW(function(c){var
+b=c[2][2];if(0===b[0])var
+e=b[1],f=aW(function(b){var
+c=g4(a,b[2]);return[0,b[1],c]},e),g=l(iO(f2),f),d=aG(ah[16],a,ah[2],g);else
+var
+d=wU(a,b[1]);return[0,c[1],d]},b),d=[0,[0,wg,l(ah[5],a)],c];return wk(ca,x(ah[34],a,d))},e);return B(function(b){return[0,b,a]},g)},wW=function(i){var
 a=i;for(;;){if(a){var
 b=a[2],d=a[1],e=d[2],f=e[2][1],j=d[1];if(f){var
 g=f[2];if(g){var
@@ -29327,7 +29388,7 @@ h=g[2];if(h){var
 c=h[2];if(c){var
 k=c[2];if(12===c[1][2][0]){if(k){var
 a=b;continue}var
-l=wU(b);return[0,[0,j,e[2]],l]}var
+l=wW(b);return[0,[0,j,e[2]],l]}var
 a=b;continue}var
 a=b;continue}var
 a=b;continue}var
@@ -29870,7 +29931,7 @@ i=a[2],g=a[1][1],V=a[4],W=a[3];if(i){var
 n=i[1],X=n[2],Y=n[1];if(i[2])return jD(g);if(W)return jD(g);var
 Z=de(c,b,X),_=aQ(function(a){if(typeof
 a!=="number"&&4===a[0]){var
-d=a[1];return f4(function(a){return de(c,jI(b,Y,a),V)},d)}return[1,[4,g,WX]]},Z);return B(function(a){return[4,a]},_)}return jD(g)}},qk=function(d,a,c,b){return[0,[0,[0,c,b],a[1]],a[2]]},iY=function(d,a,c,b){return[0,a[1],[0,[0,c,b],a[2]]]},wV=function(a){return kR(C,a[1],1,0)},mJ=function(a,c,d,b){function
+d=a[1];return f4(function(a){return de(c,jI(b,Y,a),V)},d)}return[1,[4,g,WX]]},Z);return B(function(a){return[4,a]},_)}return jD(g)}},qk=function(d,a,c,b){return[0,[0,[0,c,b],a[1]],a[2]]},iY=function(d,a,c,b){return[0,a[1],[0,[0,c,b],a[2]]]},wX=function(a){return kR(C,a[1],1,0)},mJ=function(a,c,d,b){function
 e(e,d,b){var
 f=s(Y$,s(aX(a,c,b),Y_));return s(Zb,s(e,s(Za,s(aX(a,c,d),f))))}if(typeof
 d==="number")switch(d){case
@@ -29939,78 +30000,17 @@ E=l(ah[7],a[1]);return c(_m,l(ah[7],a[1]),E);case
 2:var
 F=l(ah[7],a[1]);return c(_n,l(ah[7],a[1]),F);default:var
 G=l(ah[7],a[1]);return c(_o,l(ah[7],a[1]),G)}}var
-o=s(ZZ,s(ZY,s(aX(a,b,d),ZX)));return s(Z0,s(aX(a,b,e),o))},wW=function(c,b,d,a){return s(_q,s(aX(c,b,a),_p))},wX=function(b,a,e,d,c){var
+o=s(ZZ,s(ZY,s(aX(a,b,d),ZX)));return s(Z0,s(aX(a,b,e),o))},wY=function(c,b,d,a){return s(_q,s(aX(c,b,a),_p))},wZ=function(b,a,e,d,c){var
 f=aX(b,a,d),g=aX(b,a,c);return s(_U,s(e,s(_T,s(g,s(_S,s(f,_R))))))},mK=function(b,a,g,f,e,d,c){var
-h=aX(b,a,d),i=aX(b,a,c);return s(_0,s(g,s(_Z,s(f,s(_Y,s(i,s(_X,s(e,s(_W,s(h,_V))))))))))},wY=function(b,a,e,d,c){var
-f=aX(b,a,d),g=aX(b,a,c);return s($a,s(e,s(_$,s(g,s(__,s(f,_9))))))},wZ=function(d,c,g,f,b,a){var
-e=gj(ah[28],d,c,b,a);return e?E(e[1][1][1],0):[1,[3,f,ql(d,g,c,b,a)]]},hx=function(a,g,b,f){var
-c=b7(au,a,b);if(c){var
-d=c[1],e=d[2],h=d[1];return 0===e[0]?[0,[0,g,[0,[0,b,h],[0,b6(e[1],f)]]],a]:a}return a},g4=function(a,b){switch(b[0]){case
-0:return l(ah[5],a);case
-1:return l(ah[4],a);case
-2:return l(ah[6],a);case
-3:return l(ah[9],a);case
-4:return l(ah[10],a);case
-5:return l(ah[7],a);case
-8:return l(ah[11],a);case
-9:return l(ah[12],a);case
-10:return l(ah[13],a);case
-11:return l(ah[14],a);case
-12:return x(ah[19],a,[0,b[2],0]);case
-13:var
-c=b[2],d=l(ah[6],a),e=g4(a,c);return aG(ah[17],a,e,d);case
-14:var
-f=b[2],g=aW(function(b){var
-c=g4(a,b[2]);return[0,b[1],c]},f),h=l(iO(f2),g);return aG(ah[16],a,ah[2],h);case
-15:var
-i=g4(a,b[2]);return x(ah[15],a,i);case
-16:var
-j=b[2],k=g4(a,b[3]),m=g4(a,j);return aG(ah[17],a,m,k);default:return l(ah[8],a)}},w0=function(a,b){if(b){var
-c=w0(a,b[2]),d=l(ah[10],a);return aG(ah[17],a,d,c)}return l(ah[10],a)},k2=function(c){var
-a=r_(gs,c),e=aW(function(a){return[0,a[2],a]},a),b=aW(function(d){var
-c=d[3],b=d[2];switch(c[0]){case
-0:var
-a=iX(qd,b,0);break;case
-1:var
-a=iX(Xw,b,c[2]);break;case
-2:var
-a=iX(qd,b,c[2]);break;case
-3:var
-a=iX(Xx,b,c[2]);break;case
-4:var
-a=iX(Xy,b,c[2]);break;case
-5:var
-a=iX(Xz,b,c[2]);break;case
-8:var
-a=iX(qd,b,0);break;default:var
-a=0}return[0,d,h7(aW(function(b){var
-a=b7(au,e,b[2]);return a?[0,a[1],0]:0},a))]},a);return u_(wB,function(a){return cv(a[2])},b)},w1=function(f){var
-a=k2(f),c=0,b=em(function(b,n){var
-c=n[3],a=n[2];switch(c[0]){case
-0:return[0,[0,a,[0,[0,wg,0],[1,c[1]]]],b];case
-1:var
-d=c[3],h=c[2];return h?hx(b,a,h[1],d):au(a,mF)?[0,[0,a,[0,0,[0,d]]],b]:hx(b,a,mF,d);case
-2:var
-i=c[3],j=c[2];return j?hx(b,a,j[1],i):[0,[0,a,[0,0,[0,i]]],b];case
-3:var
-e=c[3],k=c[2];return k?hx(b,a,k[1],e):au(a,kX)?[0,[0,a,[0,0,[0,e]]],b]:hx(b,a,kX,e);case
-4:var
-f=c[3],l=c[2];return l?hx(b,a,l[1],f):au(a,mG)?[0,[0,a,[0,0,[0,f]]],b]:hx(b,a,mG,f);case
-5:var
-g=c[3],m=c[2];return m?hx(b,a,m[1],g):au(a,mH)?[0,[0,a,[0,0,[0,g]]],b]:hx(b,a,mH,g);default:return b}},a,c),d=h7(aW(function(a){var
-b=a[1],c=a[2][1];return aW(function(a){return[0,b,a]},c)},b)),e=wk(ca,l(ah[32],d)),g=aQ(function(a){var
-c=aW(function(c){var
-b=c[2][2];if(0===b[0])var
-e=b[1],f=aW(function(b){var
-c=g4(a,b[2]);return[0,b[1],c]},e),g=l(iO(f2),f),d=aG(ah[16],a,ah[2],g);else
-var
-d=w0(a,b[1]);return[0,c[1],d]},b),d=[0,[0,wg,l(ah[5],a)],c];return wk(ca,x(ah[34],a,d))},e);return B(function(b){return[0,b,a]},g)},w2=function(e,d,c,b,a){return[12,[0,c,b],d,a]},w3=function(e,c,a,l,g,d,b){var
+h=aX(b,a,d),i=aX(b,a,c);return s(_0,s(g,s(_Z,s(f,s(_Y,s(i,s(_X,s(e,s(_W,s(h,_V))))))))))},w0=function(b,a,e,d,c){var
+f=aX(b,a,d),g=aX(b,a,c);return s($a,s(e,s(_$,s(g,s(__,s(f,_9))))))},w1=function(d,c,g,f,b,a){var
+e=gj(ah[28],d,c,b,a);return e?E(e[1][1][1],0):[1,[3,f,ql(d,g,c,b,a)]]},w2=function(e,d,c,b,a){return[12,[0,c,b],d,a]},w3=function(e,c,a,l,g,d,b){var
 f=cr(e,b);if(d){var
 h=d[2],i=d[1],j=i[2],k=i[1];if(h){var
 m=aG(k,c,a,f),n=function(d){return w3(e,c,a,d,g,h,b)};return eT(function(c){return E(aG(j,a,c,b),0)},n,m)}var
-o=aG(k,c,a,f),p=function(a){return 0===a[0]?[1,l]:[1,a]};return eT(function(c){return E(aG(j,a,c,b),0)},p,o)}return[1,[3,a,wW(e,c,g,f)]]},fb=function(b,a){function
-c(b,c,d,e){return[13,[0,b,c],a,d,e]}return[0,function(c,d,e,f){return wZ(b,a,c,d,e,f)},c]},w4=function(b,a){function
-c(b,c,d,e){return[12,[0,b,c],1,[13,[0,b,c],a,d,e]]}return[0,function(c,d,e,f){return wZ(b,a,c,d,e,f)},c]},w5=function(a,c,b,k,f,e,d){var
+o=aG(k,c,a,f),p=function(a){return 0===a[0]?[1,l]:[1,a]};return eT(function(c){return E(aG(j,a,c,b),0)},p,o)}return[1,[3,a,wY(e,c,g,f)]]},fb=function(b,a){function
+c(b,c,d,e){return[13,[0,b,c],a,d,e]}return[0,function(c,d,e,f){return w1(b,a,c,d,e,f)},c]},w4=function(b,a){function
+c(b,c,d,e){return[12,[0,b,c],1,[13,[0,b,c],a,d,e]]}return[0,function(c,d,e,f){return w1(b,a,c,d,e,f)},c]},w5=function(a,c,b,k,f,e,d){var
 g=cr(a,e),h=cr(a,d);if(f){var
 i=f[1],l=f[2],m=i[2],n=gj(i[1],c,b,g,h),o=function(f){return w5(a,c,b,k,l,e,d)};return eT(function(a){return E(gj(m,b,a,e,d),0)},o,n)}var
 j=s(_t,s(_s,s(aX(a,c,h),_r)));return[1,[3,b,s(_u,s(aX(a,c,g),j))]]},cw=function(a,c,d,b){switch(b[0]){case
@@ -30035,7 +30035,7 @@ d=b[2],e=cr(a,c),f=aG(ah[22],a[1],e,d);return[0,[0,c,b[1]],f]},f)},b)},S,Q);retu
 c=b[1];return[9,[0,R,x(ah[15],a[1],b[2])],c]},T);case
 10:var
 i=b[2],u=b[1],U=cw(a,c,d,b[3]);return aQ(function(e){var
-q=[3,u,wW(a,c,i,cr(a,e))];if(i)var
+q=[3,u,wY(a,c,i,cr(a,e))];if(i)var
 b=i[1],m=0,h=[1,b],j=function(b,c,d){return w2(a,h,b,c,d)},n=[0,[0,function(e,f,d){var
 c=aG(ah[29],a,[1,b],d);return c?E(c[1][1],0):[1,[3,f,mJ(a,e,[1,b],d)]]},j],m],k=function(a,c,d){return[12,[0,a,c],[1,b],[12,[0,a,c],12,d]]},d=[0,[0,function(g,e,f){var
 c=aG(ah[29],a,12,f);if(c){var
@@ -30086,13 +30086,13 @@ ag=cw(a,c,d,D);return aQ(function(b){var
 e=cr(a,b),h=cw(a,c,iY(a[1],d,f,e),A);return B(function(c){return[15,[0,g,cr(a,c)],f,0,b,c]},h)},ag);case
 16:return wx(b[1]);case
 17:var
-o=b[1],ai=b[2],aj=E([0,0,wV(a)],0),ak=cF(function(b,e){var
+o=b[1],ai=b[2],aj=E([0,0,wX(a)],0),ak=cF(function(b,e){var
 f=cw(a,c,d,b[2]),g=aQ(function(c){var
 d=cr(a,c),e=fq(aG(ah[29],a,[0,b[1]],d),[3,o,$G],0);return B(function(a){return[0,[0,b[1],c],a[1]]},e)},f);return jC(function(c,b){var
 d=fq(gj(ah[28],a,1,b[2],c[2]),[3,o,$H],0);return B(function(a){var
 d=vl(dJ,dJ,a);return[0,[0,b[1],c[1]],d]},d)},e,g)},aj,ai);return B(function(a){return[17,[0,o,a[2]],a[1]]},ak);case
 18:var
-e=b[2],j=b[1],al=b[3],am=E([0,0,wV(a)],0),an=cF(function(b,e){var
+e=b[2],j=b[1],al=b[3],am=E([0,0,wX(a)],0),an=cF(function(b,e){var
 f=cw(a,c,d,b[2]),g=aQ(function(c){var
 d=cr(a,c),e=fq(aG(ah[29],a,[0,b[1]],d),[3,j,$I],0);return B(function(a){return[0,[0,b[1],c],a[1]]},e)},f);return jC(function(c,b){var
 d=fq(gj(ah[28],a,1,b[2],c[2]),[3,j,$J],0);return B(function(a){var
@@ -30160,10 +30160,11 @@ c=g4(a[1],b[2]);return[0,b[1],c]},f),i=cw(a,c,[0,g[1],h],e);return aQ(function(k
 d=cr(a,k),F=b[2][2];if(F){var
 e=g4(a[1],F[1]);if(bZ(C,a[1],d,e))return E([0,[0,b[1],b[2],[0,k]],g],0);var
 p=b[3],l=p?jF(p[1]):b[1],m=b[1];switch(m[0]){case
-0:return[1,[3,l,wY(a,c,m[2],d,e)]];case
+0:return[1,[3,l,w0(a,c,m[2],d,e)]];case
 1:var
-f=m[2],h=wT(a,c,d,0),i=wT(a,c,e,0),D=function(b){return wX(a,c,f,d,e)};if(0===h[0]){var
+f=m[2],h=wT(a,c,d,0),i=wT(a,c,e,0),D=function(b){return wZ(a,c,f,d,e)};if(0===h[0]){var
 n=h[1][1];if(0===i[0])var
+<<<<<<< HEAD
 <<<<<<< HEAD
 <<<<<<< HEAD
 <<<<<<< HEAD
@@ -30232,6 +30233,13 @@ j=D(i[1])}else
 var
 j=D(h[1]);return[1,[3,l,j]];default:return[1,[3,l,wY(a,c,H,d,e)]]}}return E([0,[0,b[1],b[2],[0,k]],g],0)},i)}return E([0,[0,b[1],b[2],0],g],0)},w7=function(a,d,c,b){switch(b[0]){case
 >>>>>>> Various fixes for new compiler
+=======
+o=i[1][1],q=n[2],r=n[1],s=r[2],t=r[1],u=t[2],v=t[1],w=o[2],x=o[1],y=x[2],z=x[1],A=z[2],B=z[1],G=aG(ah[23],a,v,B)?aG(ah[23],a,u,A)?aG(ah[23],a,s,y)?aG(ah[23],a,q,w)?wZ(a,c,f,d,e):mK(a,c,f,_2,_1,q,w):mK(a,c,f,_4,_3,s,y):mK(a,c,f,_6,_5,u,A):mK(a,c,f,_8,_7,v,B),j=G;else
+var
+j=D(i[1])}else
+var
+j=D(h[1]);return[1,[3,l,j]];default:return[1,[3,l,w0(a,c,H,d,e)]]}}return E([0,[0,b[1],b[2],[0,k]],g],0)},i)}return E([0,[0,b[1],b[2],0],g],0)},w7=function(a,d,c,b){switch(b[0]){case
+>>>>>>> refactor(compiler) Reorganization and renaming for internal types
 0:var
 o=b[1],p=cw(a,d,c,b[2]);return B(function(b){return[0,[0,[0,o,cr(a,b)],b],c]},p);case
 1:var
@@ -30258,6 +30266,7 @@ h=E(b,0);else{var
 <<<<<<< HEAD
 <<<<<<< HEAD
 <<<<<<< HEAD
+<<<<<<< HEAD
 k=w0(b[4]),f=[4,a,aaL],p=ht(function(a){return au(a[1],kX)?0:1},k),n=0,q=b[2],r=[0,[0,aaM,[12,a,WP]],0],t=b[3];if([0,f,0])var
 m=s(aaK,kW),i=0,j=wp(function(l,e){var
 >>>>>>> (WIP) Get the JavaScript extraction for the compiler back
@@ -30279,6 +30288,9 @@ m=s($V,kW),i=0,j=wj(function(l,e){var
 >>>>>>> Various fixes for new compiler
 =======
 k=wU(b[4]),f=[4,a,$V],p=ht(function(a){return au(a[1],kW)?0:1},k),n=0,q=b[2],r=[0,[0,$W,[12,a,VY]],0],t=b[3];if([0,f,0])var
+=======
+k=wW(b[4]),f=[4,a,$V],p=ht(function(a){return au(a[1],kW)?0:1},k),n=0,q=b[2],r=[0,[0,$W,[12,a,VY]],0],t=b[3];if([0,f,0])var
+>>>>>>> refactor(compiler) Reorganization and renaming for internal types
 m=s($U,kV),i=0,j=wj(function(l,e){var
 >>>>>>> fix(runtime) Update to JavaScript runtime; Small refactor
 g=e[2][1],p=e[1];if(g){var
@@ -30496,13 +30508,13 @@ x=qh(w,[0,h,i[1]]),j=[1,aW(function(a){return[0,a[1][1],a[2]]},x)];else
 >>>>>>> Various fixes for new compiler
 var
 j=0;var
-k=k3(c,a,d),l=k[1],y=k[2];return[0,l,kY(y,l,function(a){return wI(g,h,j,a)})];case
+k=k3(c,a,d),l=k[1],y=k[2];return[0,l,kZ(y,l,function(a){return wI(g,h,j,a)})];case
 4:var
-m=b[2],z=d4(a,m),n=k3(c,a,d),o=n[1],A=n[2],B=0;return[0,o,kY(A,o,function(a){return qe(m,z,B,a)})];case
+m=b[2],z=d4(a,m),n=k3(c,a,d),o=n[1],A=n[2],B=0;return[0,o,kZ(A,o,function(a){return qe(m,z,B,a)})];case
 5:var
-p=b[2],C=d4(a,p),q=k3(c,a,d),r=q[1],D=q[2];return[0,r,kY(D,r,function(a){return wJ(p,C,a)})];case
+p=b[2],C=d4(a,p),q=k3(c,a,d),r=q[1],D=q[2];return[0,r,kZ(D,r,function(a){return wJ(p,C,a)})];case
 6:var
-s=b[2],E=d4(a,s),t=k3(c,a,d),u=t[1],F=t[2];return[0,u,kY(F,u,function(a){return wK(s,E,a)})];default:var
+s=b[2],E=d4(a,s),t=k3(c,a,d),u=t[1],F=t[2];return[0,u,kZ(F,u,function(a){return wK(s,E,a)})];default:var
 e=d;continue}}return[0,a,c]}},xc=function(b,a){return k3(b,a[4],a[5])[2]},$_=[0,gG,[0,jB,0]],qr=function(a){return fn(au,a,$_)?1:0},$$=[0,gG,[0,jB,[0,VQ,[0,wf,[0,VR,0]]]]],eY=function(b,a){switch(a[0]){case
 0:return E([0,a[1]],0);case
 1:return E([1,a[1]],0);case
@@ -30698,7 +30710,7 @@ d=a[1],e=bP(b,a[2]);return aS(function(b,a){return[0,[0,d,b],a]},e,c)},am,ak);re
 m=a[1],ao=a[3],ap=mI(m,b,a[2]),aq=E(0,0),ar=cF(function(a,c){var
 d=a[1],e=bP(b,a[2]);return aS(function(b,a){return[0,[0,d,b],a]},e,c)},aq,ao);return aS(function(b,a){return[18,m,b,a]},ap,ar);case
 19:var
-e=a[2],f=a[1],g=e[1],as=a[3],q=b[4],at=g?kZ(wG,f,b,g[1],e[2]):wG(f,q,e[2]),au=E(0,0),av=cF(function(c,a){var
+e=a[2],f=a[1],g=e[1],as=a[3],q=b[4],at=g?k0(wG,f,b,g[1],e[2]):wG(f,q,e[2]),au=E(0,0),av=cF(function(c,a){var
 d=bP(b,c);return aS(function(b,a){return[0,b,a]},d,a)},au,as);return aS(function(b,a){return[19,f,b,a]},at,av);case
 20:var
 n=a[1],aw=a[4],ax=a[3],ay=wN(n,b,a[2]),az=E(0,0),aA=cF(function(c,a){var
@@ -30951,7 +30963,7 @@ b=mM(h,d,a[1],a[2]);return B(function(b){return[0,a[1],b]},b)},aH),aK=eY(d,aI),a
 aP=B(function(a){return[0,[0,aN,[2,o,[0,f[1],u,a]]],aM]},e);return B(function(b){var
 c=b[1],i=b[2],j=c[2],g=[0,d[1],d[2],d[3],d[4],c[1]],a=s(m,s(VO,v)),e=vw(aW(function(b){var
 c=b[1],d=c[1],f=b[2],g=c[2],e=d4(a,d);return[0,[0,d,[0,e,[0,f]]],[4,o,e,0,g]]},i)),f=e[1],k=e[2],h=em(function(c,a){var
-b=a[2],d=a[1],e=b[2],f=b[1];return jE(c,function(a){return qe(d,f,e,a)})},f,g);return[0,[0,j,k],kY(h,a,function(a){var
+b=a[2],d=a[1],e=b[2],f=b[1];return jE(c,function(a){return qe(d,f,e,a)})},f,g);return[0,[0,j,k],kZ(h,a,function(a){var
 b=a[4],c=a[3],d=b6(f,a[2]);return[0,a[1],d,c,b]})]},aP);case
 >>>>>>> (WIP) Get the JavaScript extraction for the compiler back
 3:var
@@ -31035,7 +31047,7 @@ f=b[2],c=b[1];if(0===c[0]){var
 a=c[1],g=qt(f),h=g[2],i=g[1],d=i[2],e=i[1];if(h)return[0,[0,e,[0,a,d]],h];var
 l=fn(au,a[4],$$)?1:0;return l?[0,[0,e,[0,a,d]],0]:[0,[0,e,d],[0,a]]}var
 m=c[1],j=qt(f),k=j[1];return[0,[0,[0,m,k[1]],k[2]],j[2]]}return aac},mN=function(d,c,a){var
-e=[0,c],b=[0,[2,a]];return[0,a,[0,aW(function(b){return[0,b,[0,a]]},d),b],e]},aN=function(b,a){return mN(aae,[12,a,b,[4,a,aad]],a)},eo=function(b,a){return mN(aaf,[13,a,b,[4,a,aah],[4,a,aag]],a)},aai=0,aak=[11,aaj],aam=[0,[0,aal,function(a){return aN(aak,a)}],aai],aao=[11,aan],aaq=[0,[0,aap,function(a){return aN(aao,a)}],aam],aas=[11,aar],aau=[0,[0,aat,function(a){return aN(aas,a)}],aaq],aaw=[11,aav],aay=[0,[0,aax,function(a){return aN(aaw,a)}],aau],aaA=[11,aaz],aaC=[0,[0,aaB,function(a){return aN(aaA,a)}],aay],aaE=[11,aaD],aaG=[0,[0,aaF,function(a){return aN(aaE,a)}],aaC],aaI=[11,aaH],aaK=[0,[0,aaJ,function(a){return aN(aaI,a)}],aaG],aaM=[11,aaL],aaO=[0,[0,aaN,function(a){return aN(aaM,a)}],aaK],aaQ=[11,aaP],aaS=[0,[0,aaR,function(a){return aN(aaQ,a)}],aaO],aaU=[11,aaT],aaW=[0,[0,aaV,function(a){return aN(aaU,a)}],aaS],aaY=[11,aaX],aa0=[0,[0,aaZ,function(a){return aN(aaY,a)}],aaW],aa2=[11,aa1],aa4=[0,[0,aa3,function(a){return aN(aa2,a)}],aa0],aa6=[11,aa5],aa8=[0,[0,aa7,function(a){return aN(aa6,a)}],aa4],aa_=[11,aa9],aba=[0,[0,aa$,function(a){return aN(aa_,a)}],aa8],abc=[11,abb],abe=[0,[0,abd,function(a){return aN(abc,a)}],aba],abg=[11,abf],abi=[0,[0,abh,function(a){return aN(abg,a)}],abe],abk=[11,abj],abm=[0,[0,abl,function(a){return aN(abk,a)}],abi],abo=[11,abn],abq=[0,[0,abp,function(a){return aN(abo,a)}],abm],abs=[11,abr],abu=[0,[0,abt,function(a){return aN(abs,a)}],abq],abw=[11,abv],aby=[0,[0,abx,function(a){return aN(abw,a)}],abu],abA=[11,abz],abC=[0,[0,abB,function(a){return aN(abA,a)}],aby],abE=[11,abD],abG=[0,[0,abF,function(a){return aN(abE,a)}],abC],abI=[11,abH],abK=[0,[0,abJ,function(a){return aN(abI,a)}],abG],abM=[11,abL],abO=[0,[0,abN,function(a){return aN(abM,a)}],abK],abQ=[11,abP],abS=[0,[0,abR,function(a){return aN(abQ,a)}],abO],abU=[11,abT],abW=[0,[0,abV,function(a){return aN(abU,a)}],abS],abY=[11,abX],ab0=[0,[0,abZ,function(a){return aN(abY,a)}],abW],ab2=[11,ab1],ab4=[0,[0,ab3,function(a){return aN(ab2,a)}],ab0],ab6=[11,ab5],ab8=[0,[0,ab7,function(a){return aN(ab6,a)}],ab4],ab_=[11,ab9],aca=[0,[0,ab$,function(a){return aN(ab_,a)}],ab8],acc=[11,acb],ace=[0,[0,acd,function(a){return aN(acc,a)}],aca],acg=[11,acf],aci=[0,[0,ach,function(a){return aN(acg,a)}],ace],ack=[11,acj],acm=[0,[0,acl,function(a){return aN(ack,a)}],aci],aco=[11,acn],acq=[0,[0,acp,function(a){return aN(aco,a)}],acm],acs=[11,acr],acu=[0,[0,act,function(a){return aN(acs,a)}],acq],acw=[11,acv],acy=[0,[0,acx,function(a){return aN(acw,a)}],acu],acA=[11,acz],acC=[0,[0,acB,function(a){return aN(acA,a)}],acy],acE=[11,acD],acG=[0,[0,acF,function(a){return aN(acE,a)}],acC],acI=[11,acH],acK=[0,[0,acJ,function(a){return aN(acI,a)}],acG],acM=[11,acL],acO=[0,[0,acN,function(a){return aN(acM,a)}],acK],acQ=[11,acP],acS=[0,[0,acR,function(a){return aN(acQ,a)}],acO],acT=0,acV=[3,acU],acX=[0,[0,acW,function(a){return eo(acV,a)}],acT],acZ=[3,acY],ac1=[0,[0,ac0,function(a){return eo(acZ,a)}],acX],ac3=[3,ac2],ac5=[0,[0,ac4,function(a){return eo(ac3,a)}],ac1],ac7=[3,ac6],ac9=[0,[0,ac8,function(a){return eo(ac7,a)}],ac5],ac$=[3,ac_],adb=[0,[0,ada,function(a){return eo(ac$,a)}],ac9],add=[3,adc],adf=[0,[0,ade,function(a){return eo(add,a)}],adb],adh=[3,adg],adj=[0,[0,adi,function(a){return eo(adh,a)}],adf],adl=[3,adk],adn=[0,[0,adm,function(a){return eo(adl,a)}],adj],adp=[3,ado],adr=[0,[0,adq,function(a){return eo(adp,a)}],adn],ads=[3,0],adu=b6(acS,[0,[0,adt,function(a){return eo(ads,a)}],adr]),adv=0,adx=[11,adw],adz=[0,[0,ady,function(a){return aN(adx,a)}],adv],adB=[11,adA],adD=[0,[0,adC,function(a){return aN(adB,a)}],adz],adE=3,adG=[0,[0,adF,function(a){return aN(adE,a)}],adD],adH=4,adJ=[0,[0,adI,function(a){return aN(adH,a)}],adG],adK=6,adM=[0,[0,adL,function(a){return aN(adK,a)}],adJ],adN=5,adP=[0,[0,adO,function(a){return aN(adN,a)}],adM],adQ=18,adS=[0,[0,adR,function(a){return aN(adQ,a)}],adP],adT=18,adV=[0,[0,adU,function(a){return aN(adT,a)}],adS],adW=18,adY=[0,[0,adX,function(a){return aN(adW,a)}],adV],adZ=19,ad1=[0,[0,ad0,function(a){return aN(adZ,a)}],adY],ad2=20,ad4=[0,[0,ad3,function(a){return aN(ad2,a)}],ad1],ad5=21,ad7=[0,[0,ad6,function(a){return aN(ad5,a)}],ad4],ad8=22,ad_=[0,[0,ad9,function(a){return aN(ad8,a)}],ad7],aeb=[0,[0,aea,function(a){return aN(ad$,a)}],ad_],aee=[0,[0,aed,function(a){return aN(aec,a)}],aeb],aeh=[0,[0,aeg,function(a){return aN(aef,a)}],aee],aek=[0,[0,aej,function(a){return aN(aei,a)}],aeh],aen=[0,[0,aem,function(a){return aN(ael,a)}],aek],aeq=[0,[0,aep,function(a){return aN(aeo,a)}],aen],aet=[0,[0,aes,function(a){return aN(aer,a)}],aeq],aeu=17,aew=[0,[0,aev,function(a){return aN(aeu,a)}],aet],aez=[0,[0,aey,function(a){return aN(aex,a)}],aew],aeC=[0,[0,aeB,function(a){return aN(aeA,a)}],aez],aeF=[0,[0,aeE,function(a){return aN(aeD,a)}],aeC],aeG=17,aeI=[0,[0,aeH,function(a){return aN(aeG,a)}],aeF],aeL=[0,[0,aeK,function(a){return aN(aeJ,a)}],aeI],aeO=[0,[0,aeN,function(a){return aN(aeM,a)}],aeL],aeR=[0,[0,aeQ,function(a){return aN(aeP,a)}],aeO],aeT=[11,aeS],aeV=[0,[0,aeU,function(a){return aN(aeT,a)}],aeR],aeX=[11,aeW],aeZ=[0,[0,aeY,function(a){return aN(aeX,a)}],aeV],ae0=9,ae2=[0,[0,ae1,function(a){return aN(ae0,a)}],aeZ],ae3=8,ae5=[0,[0,ae4,function(a){return aN(ae3,a)}],ae2],ae6=7,ae8=[0,[0,ae7,function(a){return aN(ae6,a)}],ae5],ae9=[11,0],ae$=[0,[0,ae_,function(a){return aN(ae9,a)}],ae8],afa=0,afb=14,afd=[0,[0,afc,function(a){return eo(afb,a)}],afa],afe=12,afg=[0,[0,aff,function(a){return eo(afe,a)}],afd],afh=8,afj=[0,[0,afi,function(a){return eo(afh,a)}],afg],afk=7,afm=[0,[0,afl,function(a){return eo(afk,a)}],afj],afp=[0,[0,afo,function(a){return eo(afn,a)}],afm],afs=[0,[0,afr,function(a){return eo(afq,a)}],afp],afv=[0,[0,afu,function(a){return eo(aft,a)}],afs],afy=[0,[0,afx,function(a){return eo(afw,a)}],afv],afB=[0,[0,afA,function(a){return eo(afz,a)}],afy],afE=[0,[0,afD,function(a){return eo(afC,a)}],afB],afF=0,afH=[0,[0,afG,function(a){return mN(0,[4,a,p6],a)}],afF],afJ=[0,[0,afI,function(a){return mN(0,[4,a,p5],a)}],afH],afK=b6(adu,b6(afJ,b6(ae$,afE))),xg=function(c,a,b){return[0,b,a[2],a[3],a[4],a[5],a[6],a[7],a[8],a[9],a[10],a[11],a[12],a[13]]},xh=function(d,a,c,b){return[0,a[1],a[2],a[3],a[4],a[5],a[6],[0,c],a[8],a[9],a[10],a[11],a[12],b]},qu=function(c,a,b){return[0,a[1],a[2],a[3],a[4],a[5],a[6],a[7],a[8],b,a[10],a[11],a[12],a[13]]},xi=function(b,a){return k2(b6(a[10],a[11]))},bY=function(c,b,a){switch(a[0]){case
+e=[0,c],b=[0,[2,a]];return[0,a,[0,aW(function(b){return[0,b,[0,a]]},d),b],e]},aN=function(b,a){return mN(aae,[12,a,b,[4,a,aad]],a)},eo=function(b,a){return mN(aaf,[13,a,b,[4,a,aah],[4,a,aag]],a)},aai=0,aak=[11,aaj],aam=[0,[0,aal,function(a){return aN(aak,a)}],aai],aao=[11,aan],aaq=[0,[0,aap,function(a){return aN(aao,a)}],aam],aas=[11,aar],aau=[0,[0,aat,function(a){return aN(aas,a)}],aaq],aaw=[11,aav],aay=[0,[0,aax,function(a){return aN(aaw,a)}],aau],aaA=[11,aaz],aaC=[0,[0,aaB,function(a){return aN(aaA,a)}],aay],aaE=[11,aaD],aaG=[0,[0,aaF,function(a){return aN(aaE,a)}],aaC],aaI=[11,aaH],aaK=[0,[0,aaJ,function(a){return aN(aaI,a)}],aaG],aaM=[11,aaL],aaO=[0,[0,aaN,function(a){return aN(aaM,a)}],aaK],aaQ=[11,aaP],aaS=[0,[0,aaR,function(a){return aN(aaQ,a)}],aaO],aaU=[11,aaT],aaW=[0,[0,aaV,function(a){return aN(aaU,a)}],aaS],aaY=[11,aaX],aa0=[0,[0,aaZ,function(a){return aN(aaY,a)}],aaW],aa2=[11,aa1],aa4=[0,[0,aa3,function(a){return aN(aa2,a)}],aa0],aa6=[11,aa5],aa8=[0,[0,aa7,function(a){return aN(aa6,a)}],aa4],aa_=[11,aa9],aba=[0,[0,aa$,function(a){return aN(aa_,a)}],aa8],abc=[11,abb],abe=[0,[0,abd,function(a){return aN(abc,a)}],aba],abg=[11,abf],abi=[0,[0,abh,function(a){return aN(abg,a)}],abe],abk=[11,abj],abm=[0,[0,abl,function(a){return aN(abk,a)}],abi],abo=[11,abn],abq=[0,[0,abp,function(a){return aN(abo,a)}],abm],abs=[11,abr],abu=[0,[0,abt,function(a){return aN(abs,a)}],abq],abw=[11,abv],aby=[0,[0,abx,function(a){return aN(abw,a)}],abu],abA=[11,abz],abC=[0,[0,abB,function(a){return aN(abA,a)}],aby],abE=[11,abD],abG=[0,[0,abF,function(a){return aN(abE,a)}],abC],abI=[11,abH],abK=[0,[0,abJ,function(a){return aN(abI,a)}],abG],abM=[11,abL],abO=[0,[0,abN,function(a){return aN(abM,a)}],abK],abQ=[11,abP],abS=[0,[0,abR,function(a){return aN(abQ,a)}],abO],abU=[11,abT],abW=[0,[0,abV,function(a){return aN(abU,a)}],abS],abY=[11,abX],ab0=[0,[0,abZ,function(a){return aN(abY,a)}],abW],ab2=[11,ab1],ab4=[0,[0,ab3,function(a){return aN(ab2,a)}],ab0],ab6=[11,ab5],ab8=[0,[0,ab7,function(a){return aN(ab6,a)}],ab4],ab_=[11,ab9],aca=[0,[0,ab$,function(a){return aN(ab_,a)}],ab8],acc=[11,acb],ace=[0,[0,acd,function(a){return aN(acc,a)}],aca],acg=[11,acf],aci=[0,[0,ach,function(a){return aN(acg,a)}],ace],ack=[11,acj],acm=[0,[0,acl,function(a){return aN(ack,a)}],aci],aco=[11,acn],acq=[0,[0,acp,function(a){return aN(aco,a)}],acm],acs=[11,acr],acu=[0,[0,act,function(a){return aN(acs,a)}],acq],acw=[11,acv],acy=[0,[0,acx,function(a){return aN(acw,a)}],acu],acA=[11,acz],acC=[0,[0,acB,function(a){return aN(acA,a)}],acy],acE=[11,acD],acG=[0,[0,acF,function(a){return aN(acE,a)}],acC],acI=[11,acH],acK=[0,[0,acJ,function(a){return aN(acI,a)}],acG],acM=[11,acL],acO=[0,[0,acN,function(a){return aN(acM,a)}],acK],acQ=[11,acP],acS=[0,[0,acR,function(a){return aN(acQ,a)}],acO],acT=0,acV=[3,acU],acX=[0,[0,acW,function(a){return eo(acV,a)}],acT],acZ=[3,acY],ac1=[0,[0,ac0,function(a){return eo(acZ,a)}],acX],ac3=[3,ac2],ac5=[0,[0,ac4,function(a){return eo(ac3,a)}],ac1],ac7=[3,ac6],ac9=[0,[0,ac8,function(a){return eo(ac7,a)}],ac5],ac$=[3,ac_],adb=[0,[0,ada,function(a){return eo(ac$,a)}],ac9],add=[3,adc],adf=[0,[0,ade,function(a){return eo(add,a)}],adb],adh=[3,adg],adj=[0,[0,adi,function(a){return eo(adh,a)}],adf],adl=[3,adk],adn=[0,[0,adm,function(a){return eo(adl,a)}],adj],adp=[3,ado],adr=[0,[0,adq,function(a){return eo(adp,a)}],adn],ads=[3,0],adu=b6(acS,[0,[0,adt,function(a){return eo(ads,a)}],adr]),adv=0,adx=[11,adw],adz=[0,[0,ady,function(a){return aN(adx,a)}],adv],adB=[11,adA],adD=[0,[0,adC,function(a){return aN(adB,a)}],adz],adE=3,adG=[0,[0,adF,function(a){return aN(adE,a)}],adD],adH=4,adJ=[0,[0,adI,function(a){return aN(adH,a)}],adG],adK=6,adM=[0,[0,adL,function(a){return aN(adK,a)}],adJ],adN=5,adP=[0,[0,adO,function(a){return aN(adN,a)}],adM],adQ=18,adS=[0,[0,adR,function(a){return aN(adQ,a)}],adP],adT=18,adV=[0,[0,adU,function(a){return aN(adT,a)}],adS],adW=18,adY=[0,[0,adX,function(a){return aN(adW,a)}],adV],adZ=19,ad1=[0,[0,ad0,function(a){return aN(adZ,a)}],adY],ad2=20,ad4=[0,[0,ad3,function(a){return aN(ad2,a)}],ad1],ad5=21,ad7=[0,[0,ad6,function(a){return aN(ad5,a)}],ad4],ad8=22,ad_=[0,[0,ad9,function(a){return aN(ad8,a)}],ad7],aeb=[0,[0,aea,function(a){return aN(ad$,a)}],ad_],aee=[0,[0,aed,function(a){return aN(aec,a)}],aeb],aeh=[0,[0,aeg,function(a){return aN(aef,a)}],aee],aek=[0,[0,aej,function(a){return aN(aei,a)}],aeh],aen=[0,[0,aem,function(a){return aN(ael,a)}],aek],aeq=[0,[0,aep,function(a){return aN(aeo,a)}],aen],aet=[0,[0,aes,function(a){return aN(aer,a)}],aeq],aeu=17,aew=[0,[0,aev,function(a){return aN(aeu,a)}],aet],aez=[0,[0,aey,function(a){return aN(aex,a)}],aew],aeC=[0,[0,aeB,function(a){return aN(aeA,a)}],aez],aeF=[0,[0,aeE,function(a){return aN(aeD,a)}],aeC],aeG=17,aeI=[0,[0,aeH,function(a){return aN(aeG,a)}],aeF],aeL=[0,[0,aeK,function(a){return aN(aeJ,a)}],aeI],aeO=[0,[0,aeN,function(a){return aN(aeM,a)}],aeL],aeR=[0,[0,aeQ,function(a){return aN(aeP,a)}],aeO],aeT=[11,aeS],aeV=[0,[0,aeU,function(a){return aN(aeT,a)}],aeR],aeX=[11,aeW],aeZ=[0,[0,aeY,function(a){return aN(aeX,a)}],aeV],ae0=9,ae2=[0,[0,ae1,function(a){return aN(ae0,a)}],aeZ],ae3=8,ae5=[0,[0,ae4,function(a){return aN(ae3,a)}],ae2],ae6=7,ae8=[0,[0,ae7,function(a){return aN(ae6,a)}],ae5],ae9=[11,0],ae$=[0,[0,ae_,function(a){return aN(ae9,a)}],ae8],afa=0,afb=14,afd=[0,[0,afc,function(a){return eo(afb,a)}],afa],afe=12,afg=[0,[0,aff,function(a){return eo(afe,a)}],afd],afh=8,afj=[0,[0,afi,function(a){return eo(afh,a)}],afg],afk=7,afm=[0,[0,afl,function(a){return eo(afk,a)}],afj],afp=[0,[0,afo,function(a){return eo(afn,a)}],afm],afs=[0,[0,afr,function(a){return eo(afq,a)}],afp],afv=[0,[0,afu,function(a){return eo(aft,a)}],afs],afy=[0,[0,afx,function(a){return eo(afw,a)}],afv],afB=[0,[0,afA,function(a){return eo(afz,a)}],afy],afE=[0,[0,afD,function(a){return eo(afC,a)}],afB],afF=0,afH=[0,[0,afG,function(a){return mN(0,[4,a,p6],a)}],afF],afJ=[0,[0,afI,function(a){return mN(0,[4,a,p5],a)}],afH],afK=b6(adu,b6(afJ,b6(ae$,afE))),xg=function(c,a,b){return[0,b,a[2],a[3],a[4],a[5],a[6],a[7],a[8],a[9],a[10],a[11],a[12],a[13]]},xh=function(d,a,c,b){return[0,a[1],a[2],a[3],a[4],a[5],a[6],[0,c],a[8],a[9],a[10],a[11],a[12],b]},qu=function(c,a,b){return[0,a[1],a[2],a[3],a[4],a[5],a[6],a[7],a[8],b,a[10],a[11],a[12],a[13]]},xi=function(b,a){return kY(b6(a[10],a[11]))},bY=function(c,b,a){switch(a[0]){case
 0:var
 h=a[1];return b[7]?E(w8(h),0):wm(h);case
 1:var
@@ -31734,8 +31746,12 @@ j=b[2],k=j[2],C=b[1];if(fn(au,k,aW(wz,a[11])))return[1,[2,C,s(afR,s(k,afQ))]];va
 o=a[13],p=a[12],q=k3(b6(a[11],[0,j,0]));return E([0,0,[0,a[1],a[2],a[3],a[4],a[5],a[6],a[7],a[8],a[9],a[10],q,p,o]],0);case
 =======
 j=b[2],k=j[2],C=b[1];if(fn(au,k,aW(wB,a[11])))return[1,[2,C,s(afS,s(k,afR))]];var
+<<<<<<< HEAD
 o=a[13],p=a[12],q=k2(b6(a[11],[0,j,0]));return E([0,0,[0,a[1],a[2],a[3],a[4],a[5],a[6],a[7],a[8],a[9],a[10],q,p,o]],0);case
 >>>>>>> fix(runtime) Update to JavaScript runtime; Small refactor
+=======
+o=a[13],p=a[12],q=kY(b6(a[11],[0,j,0]));return E([0,0,[0,a[1],a[2],a[3],a[4],a[5],a[6],a[7],a[8],a[9],a[10],q,p,o]],0);case
+>>>>>>> refactor(compiler) Reorganization and renaming for internal types
 3:var
 l=b[1],z=fr(d,a,b[2]),A=B(function(a){return w8(l,a)},z),D=B(function(a){return[0,l,a]},A);return B(function(b){return[0,[0,b,0],a]},D);case
 >>>>>>> (WIP) Switch back to new backend CodeGeneration for JS
@@ -61827,9 +61843,14 @@ at9=function(a){return[0,0,1,0,0,0,0,0,0,0]},yO=function(a,c,b){a[4]=[0,[0,c,b],
 b=u8(yM,xE),c=u8(yN,xD),d=cl(xD,xE);a[4]=cl(d,a[4]);a[6]=cl(c,a[6]);a[7]=cl(b,a[7]);return 0},aud=function(D,b,h){try{var
 a=at1(auf,h),c=[0,aug,b],d=gw(function(r,F){var
 t=r[2],o=k6[1],c=t[2],G=r[1];if(c[11])var
+<<<<<<< HEAD
 m=b6(c[10],c[11]),C=w1(m),n=B(function(f){var
 g=f[1],a=c[13],b=c[12],d=k2(0),e=k2(m);return[0,g,[0,c[1],c[2],c[3],c[4],c[5],c[6],c[7],c[8],c[9],e,d,b,a]]},C);else
 >>>>>>> fix(runtime) Update to JavaScript runtime; Small refactor
+=======
+m=b6(c[10],c[11]),C=wV(m),n=B(function(f){var
+g=f[1],a=c[13],b=c[12],d=kY(0),e=kY(m);return[0,g,[0,c[1],c[2],c[3],c[4],c[5],c[6],c[7],c[8],c[9],e,d,b,a]]},C);else
+>>>>>>> refactor(compiler) Reorganization and renaming for internal types
 var
 n=E([0,o,c],0);var
 g=B(function(a){var
@@ -61971,7 +61992,7 @@ var
 p=Y5,an=0;var
 bQ=p[2],bR=p[1],bS=g3(a,b,f,bL,an),bT=s(g1(a,b,bN,bR),bS),e=s(g2(a,b,bM,bQ),bT)}else
 var
-e=eF(b,c)}return s(e,k0)}return 0},z),i=[0,A,eT(h6,function(a){return e},k)]}else
+e=eF(b,c)}return s(e,k1)}return 0},z),i=[0,A,eT(h6,function(a){return e},k)]}else
 var
 i=fc(g[1]);var
 H=i[2],I=i[1],J=D[9];return[0,aw(G,xu(function(a,b){if(J)e8(function(b){var
@@ -61996,7 +62017,7 @@ e=[0,yN(c,b),0];a[6]=cl(a[6],e);return 0},z);e8(function(d){var
 b=d[2],c=d[1];yO(a,c,b);var
 e=[0,yM(c,b),0];a[7]=cl(a[7],e);return 0},y);if(j){var
 o=j[1],m=o[2],g=o[1];a[3]=[0,[0,g,m]];fL[1]=g;a[5]=[0,[0,g,qE(at0,m)]]}var
-A=a[7],C=cy(function(a){return[0,a]},A),D=a[6],k=agP(cl(cy(function(a){return[1,a]},D),C)),c=aQ(w1,B(XD,B(dJ,xp(k,0))));if(0===c[0]){k6[1]=c[1][1][1];var
+A=a[7],C=cy(function(a){return[0,a]},A),D=a[6],k=agP(cl(cy(function(a){return[1,a]},D),C)),c=aQ(wV,B(XD,B(dJ,xp(k,0))));if(0===c[0]){k6[1]=c[1][1][1];var
 b=k6[1],t=0,p=xp(k,0),q=B(function(c){var
 a=b[1],i=c[2],j=c[1],d=l(ah[4],a),e=[0,[0,hw,x(ah[15],a,d)],0],f=[0,[0,fI,l(ah[6],a)],e],g=[0,[0,iV,l(ah[6],a)],f],h=[0,[0,p5,l(ah[12],a)],g];return[0,j,[0,i,0,0,0,0,0,0,0,[0,[0,[0,p6,x(ah[19],a,[0,wh,0])],h],0],t,0,0,0]]},p),r=function(a){var
 d=a[2],e=a[1];function
@@ -62016,7 +62037,7 @@ n=fc(c[1]);var
 I=xu(function(a,b){return a},n);jd(jc,aw(auc,aw(qy,aub)));function
 K(e,d,c){var
 b=aud(a,d,gL(c));return{"out":b[1].toString(),"ctx":b[2]}}var
-L={"initRCtxt":I,"version":qy.toString(),"buildate":"Jan 26, 2020","runLine":avb(K)};return ava(0).ergotop=L},aur=function(g,a){var
+L={"initRCtxt":I,"version":qy.toString(),"buildate":"Jan 29, 2020","runLine":avb(K)};return ava(0).ergotop=L},aur=function(g,a){var
 o=g[3],p=o?[0,o[1],g[4]]:g[4];if(a[1]===mR)return new
 s6(qx(p,a[2]).toString());function
 t(e){var
