compiler/core/ErgoC/Lang/ErgoCTypecheck.v
@@ -24,8 +24,8 @@ Require Import ErgoSpec.Common.Result.
 Require Import ErgoSpec.Common.Provenance.
 Require Import ErgoSpec.Common.Ast.
 Require Import ErgoSpec.Common.PrintTypedData.
-Require Import ErgoSpec.Types.ErgoCTypeUtil.
-Require Import ErgoSpec.Types.ErgoTypetoErgoCType.
+Require Import ErgoSpec.Types.QcertTypeUtil.
+Require Import ErgoSpec.Types.ErgoTypetoQcertType.
 Require Import ErgoSpec.Ergo.Lang.Ergo.
 Require Import ErgoSpec.ErgoC.Lang.ErgoC.
 Require Import ErgoSpec.ErgoC.Lang.ErgoCOverloaded.
@@ -37,7 +37,7 @@ Section ErgoCTypecheck.
 
   Import QcertType.
 
-  Fixpoint ergoc_typecheck_expr nsctxt (ctxt : type_context) (expr : ergoc_expr) : eresult ergoct_expr :=
+  Fixpoint ergoc_expr_typecheck nsctxt (ctxt : type_context) (expr : ergoc_expr) : eresult ergoct_expr :=
     match expr with
     | EThis prov => this_in_calculus_error prov
     | EThisContract prov => contract_in_calculus_error prov
@@ -53,64 +53,64 @@ Section ErgoCTypecheck.
     | EText prov _ => text_in_calculus_error prov
     | ENone prov => esuccess (ENone (prov, toption tbottom)) nil
     | ESome prov e =>
-      elift (fun eT => ESome (prov,toption (exprct_type_annot eT)) eT) (ergoc_typecheck_expr nsctxt ctxt e)
+      elift (fun eT => ESome (prov,toption (exprct_type_annot eT)) eT) (ergoc_expr_typecheck nsctxt ctxt e)
     | EArray prov es =>
       elift (fun eT => EArray (prov,tcoll (snd eT)) (fst eT))
             (fold_right
-               (fun (new:ergoc_expr) (eT:eresult (list ergoct_expr * ergoc_type)) =>
+               (fun (new:ergoc_expr) (eT:eresult (list ergoct_expr * qcert_type)) =>
                   eolift
-                    (fun (eT':list ergoct_expr * ergoc_type) =>
+                    (fun (eT':list ergoct_expr * qcert_type) =>
                        elift
                          (fun (new':ergoct_expr) =>
-                            (new'::(fst eT'), ergoc_type_join (exprct_type_annot new') (snd eT')))
-                         (ergoc_typecheck_expr nsctxt ctxt new))
+                            (new'::(fst eT'), qcert_type_join (exprct_type_annot new') (snd eT')))
+                         (ergoc_expr_typecheck nsctxt ctxt new))
                     eT)
                (esuccess (nil,tbottom) nil) es)
     | EUnaryOperator prov eop e =>
       eolift (unary_dispatch nsctxt prov eop)
-             (ergoc_typecheck_expr nsctxt ctxt e)
+             (ergoc_expr_typecheck nsctxt ctxt e)
     | EBinaryOperator prov eop e1 e2 =>
       eolift2 (binary_dispatch nsctxt prov eop)
-              (ergoc_typecheck_expr nsctxt ctxt e1)
-              (ergoc_typecheck_expr nsctxt ctxt e2)
+              (ergoc_expr_typecheck nsctxt ctxt e1)
+              (ergoc_expr_typecheck nsctxt ctxt e2)
     | EUnaryBuiltin prov op e =>
       eolift
         (fun eT =>
            let t := exprct_type_annot eT in
-           match ergoc_type_infer_unary_op op t with
+           match qcert_type_infer_unary_op op t with
            | Some (r, _) => esuccess (EUnaryBuiltin (prov,r) op eT) nil
            | None => efailure (ETypeError prov (ergo_format_unop_error nsctxt op t))
            end)
-        (ergoc_typecheck_expr nsctxt ctxt e)
+        (ergoc_expr_typecheck nsctxt ctxt e)
     | EBinaryBuiltin prov op e1 e2 =>
       eolift2
         (fun eT1 eT2 =>
           let t1 := exprct_type_annot eT1 in
           let t2 := exprct_type_annot eT2 in
-          match ergoc_type_infer_binary_op op t1 t2 with
+          match qcert_type_infer_binary_op op t1 t2 with
           | Some (r, _, _) => esuccess (EBinaryBuiltin (prov,r) op eT1 eT2) nil
           | None => efailure (ETypeError prov (ergo_format_binop_error nsctxt op t1 t2))
           end)
-        (ergoc_typecheck_expr nsctxt ctxt e1)
-        (ergoc_typecheck_expr nsctxt ctxt e2)
+        (ergoc_expr_typecheck nsctxt ctxt e1)
+        (ergoc_expr_typecheck nsctxt ctxt e2)
     | EIf prov c t f =>
       eolift (fun cT' =>
-                if ergoc_type_subtype_dec (exprct_type_annot cT') tbool then
+                if qcert_type_subtype_dec (exprct_type_annot cT') tbool then
                   elift2 (fun eT1 eT2 =>
                             let t1 := exprct_type_annot eT1 in
                             let t2 := exprct_type_annot eT2 in
-                            EIf (prov,ergoc_type_join t1 t2) cT' eT1 eT2)
-                         (ergoc_typecheck_expr nsctxt ctxt t)
-                         (ergoc_typecheck_expr nsctxt ctxt f)
+                            EIf (prov,qcert_type_join t1 t2) cT' eT1 eT2)
+                         (ergoc_expr_typecheck nsctxt ctxt t)
+                         (ergoc_expr_typecheck nsctxt ctxt f)
                 else efailure (ETypeError (expr_annot c) "'if' condition not boolean."%string))
-             (ergoc_typecheck_expr nsctxt ctxt c)
+             (ergoc_expr_typecheck nsctxt ctxt c)
     | ELet prov n None v e =>
       (eolift (fun evT =>
                  let vt := exprct_type_annot evT in
                  let ctxt' := type_context_update_local_env ctxt n vt in
                  elift (fun eT => ELet (prov, exprct_type_annot eT) n None evT eT)
-                       (ergoc_typecheck_expr nsctxt ctxt' e))
-              (ergoc_typecheck_expr nsctxt ctxt v))
+                       (ergoc_expr_typecheck nsctxt ctxt' e))
+              (ergoc_expr_typecheck nsctxt ctxt v))
     | ELet prov n (Some t) v e  =>
       let fmt_err :=
           fun t' vt =>
@@ -121,24 +121,24 @@ Section ErgoCTypecheck.
                                      ++ "' expected argument `"
                                      ++ n
                                      ++ "' to be of type `"
-                                     ++ (ergoc_type_to_string nsctxt t')
+                                     ++ (qcert_type_to_string nsctxt t')
                                      ++ "' but was given argument of type `"
-                                     ++ (ergoc_type_to_string nsctxt vt)
+                                     ++ (qcert_type_to_string nsctxt vt)
                                      ++ "'." )
           | _ => ETypeError prov
                             ("The let type annotation `"
-                               ++ (ergoc_type_to_string nsctxt t')
+                               ++ (qcert_type_to_string nsctxt t')
                                ++ "' for the name `"
                                ++ n
                                ++ "' does not match the actual type `"
-                               ++ (ergoc_type_to_string nsctxt vt)
+                               ++ (qcert_type_to_string nsctxt vt)
                                ++ "'.")
           end
       in
       (eolift
          (fun evT =>
             let vt := exprct_type_annot evT in
-            let t' := (ergo_type_to_ergoc_type t) in
+            let t' := (ergo_type_to_qcert_type t) in
             if subtype_dec vt t' then
               let ctxt' :=
                   type_context_update_local_env
@@ -146,31 +146,31 @@ Section ErgoCTypecheck.
                     t'
               in
               elift (fun eT => ELet (prov, exprct_type_annot eT) n (Some t) evT eT)
-                    (ergoc_typecheck_expr nsctxt ctxt' e)
+                    (ergoc_expr_typecheck nsctxt ctxt' e)
             else
               efailure (fmt_err t' vt))
-         (ergoc_typecheck_expr nsctxt ctxt v))
+         (ergoc_expr_typecheck nsctxt ctxt v))
     | EPrint prov v e =>
       print_in_calculus_error prov
     | ERecord prov rs =>
       elift (fun eT => ERecord (prov,(snd eT)) (fst eT))
             (fold_right
-               (fun (next:string * ergoc_expr) (sofar:eresult (list (string * ergoct_expr) * ergoc_type)) =>
+               (fun (next:string * ergoc_expr) (sofar:eresult (list (string * ergoct_expr) * qcert_type)) =>
                   eolift2
-                    (fun (sofar':list (string * ergoct_expr) * ergoc_type)
-                         (next':(string * ergoct_expr) * ergoc_type) =>
+                    (fun (sofar':list (string * ergoct_expr) * qcert_type)
+                         (next':(string * ergoct_expr) * qcert_type) =>
                        elift (fun T' => (fst next'::fst sofar',compose fst fst T'))
                              (eresult_of_option
-                                (ergoc_type_infer_binary_op OpRecConcat (snd next') (snd sofar'))
+                                (qcert_type_infer_binary_op OpRecConcat (snd next') (snd sofar'))
                                 (ETypeError prov "Bad record! Failed to concat."%string) nil))
                     sofar
                     (eolift (fun efT =>
                                let ft := exprct_type_annot efT in
                                elift (fun T => ((fst next,efT), fst T))
                                      (eresult_of_option
-                                        (ergoc_type_infer_unary_op (OpRec (fst next)) ft)
+                                        (qcert_type_infer_unary_op (OpRec (fst next)) ft)
                                         (ETypeError prov "Bad record! Failed to init."%string) nil))
-                            (ergoc_typecheck_expr nsctxt ctxt (snd next))))
+                            (ergoc_expr_typecheck nsctxt ctxt (snd next))))
                (esuccess (nil,empty_rec_type) nil) rs)
     | ENew prov name rs =>
       eolift
@@ -180,22 +180,22 @@ Section ErgoCTypecheck.
                     (infer_brand_strict (name::nil) (snd rsT'))
                     (ETypeError prov (ergo_format_new_error nsctxt name (snd rsT'))) nil))
         (fold_right
-           (fun (next:string * ergoc_expr) (sofar:eresult (list (string * ergoct_expr) * ergoc_type)) =>
+           (fun (next:string * ergoc_expr) (sofar:eresult (list (string * ergoct_expr) * qcert_type)) =>
               eolift2
-                (fun (sofar':list (string * ergoct_expr) * ergoc_type)
-                     (next':(string * ergoct_expr) * ergoc_type) =>
+                (fun (sofar':list (string * ergoct_expr) * qcert_type)
+                     (next':(string * ergoct_expr) * qcert_type) =>
                    elift (fun T' => (fst next'::fst sofar',compose fst fst T'))
                          (eresult_of_option
-                            (ergoc_type_infer_binary_op OpRecConcat (snd next') (snd sofar'))
+                            (qcert_type_infer_binary_op OpRecConcat (snd next') (snd sofar'))
                             (ETypeError prov "Bad record! Failed to concat."%string) nil))
                 sofar
                 (eolift (fun efT =>
                            let ft := exprct_type_annot efT in
                            elift (fun T => ((fst next,efT), fst T))
                                  (eresult_of_option
-                                    (ergoc_type_infer_unary_op (OpRec (fst next)) ft)
+                                    (qcert_type_infer_unary_op (OpRec (fst next)) ft)
                                     (ETypeError prov "Bad record! Failed to init."%string) nil))
-                        (ergoc_typecheck_expr nsctxt ctxt (snd next))))
+                        (ergoc_expr_typecheck nsctxt ctxt (snd next))))
            (esuccess (nil,empty_rec_type) nil) rs)
     | ECallFun prov fname args => function_not_inlined_error prov "typing" fname
     | ECallFunInGroup prov gname fname args => function_in_group_not_inlined_error prov gname fname
@@ -214,15 +214,15 @@ Section ErgoCTypecheck.
                (fun pe sofarT =>
                   match pe with
                   | (CaseData prov d, res) => (* TODO can `d' ever be bad? *)
-                    match ergoc_type_infer_data d with
+                    match qcert_type_infer_data d with
                     | None => efailure (ETypeError prov "Ill-typed data literal!")
                     | Some dt =>
                       elift2 (fun sofarT eT =>
                                 let et := exprct_type_annot eT in
-                                let sofart := ergoc_type_join et (snd sofarT) in
+                                let sofart := qcert_type_join et (snd sofarT) in
                                 ((CaseData (prov,sofart) d,eT)::fst sofarT, sofart))
                              sofarT
-                             (ergoc_typecheck_expr nsctxt ctxt res)
+                             (ergoc_expr_typecheck nsctxt ctxt res)
                     end
                   | (CaseEnum prov name, res) =>
                     let opt := lookup String.string_dec (ctxt.(type_context_local_env)++ctxt.(type_context_global_env)) name in
@@ -230,32 +230,32 @@ Section ErgoCTypecheck.
                     eolift (fun dt =>
                              elift2 (fun sofarT eT =>
                                        let et := exprct_type_annot eT in
-                                       let sofart := ergoc_type_join et (snd sofarT) in
+                                       let sofart := qcert_type_join et (snd sofarT) in
                                        ((CaseEnum (prov,sofart) name,eT)::fst sofarT, sofart))
                                     sofarT
-                                    (ergoc_typecheck_expr nsctxt ctxt res))
+                                    (ergoc_expr_typecheck nsctxt ctxt res))
                            topt
                   | (CaseWildcard prov None, res) =>
                     elift2 (fun sofarT eT =>
                               let et := exprct_type_annot eT in
-                              let sofart := ergoc_type_join et (snd sofarT) in
+                              let sofart := qcert_type_join et (snd sofarT) in
                               ((CaseWildcard (prov,sofart) None,eT)::fst sofarT, sofart))
                            sofarT
-                           (ergoc_typecheck_expr nsctxt ctxt res)
+                           (ergoc_expr_typecheck nsctxt ctxt res)
                   | (CaseLet prov name None, res) =>
                     elift2 (fun sofarT eT =>
                               let et := exprct_type_annot eT in
-                              let sofart := ergoc_type_join et (snd sofarT) in
+                              let sofart := qcert_type_join et (snd sofarT) in
                               ((CaseLet (prov,sofart) name None,eT)::fst sofarT, sofart))
                            sofarT
-                           (ergoc_typecheck_expr nsctxt (type_context_update_local_env ctxt name t0) res)
+                           (ergoc_expr_typecheck nsctxt (type_context_update_local_env ctxt name t0) res)
                   | (CaseLet prov name (Some b), res) =>
                     elift2 (fun sofarT eT =>
                               let et := exprct_type_annot eT in
-                              let sofart := ergoc_type_join et (snd sofarT) in
+                              let sofart := qcert_type_join et (snd sofarT) in
                               ((CaseLet (prov,sofart) name (Some b), eT)::fst sofarT, sofart))
                            sofarT
-                           (ergoc_typecheck_expr
+                           (ergoc_expr_typecheck
                               nsctxt
                               (type_context_update_local_env
                                  ctxt
@@ -269,10 +269,10 @@ Section ErgoCTypecheck.
                     | Some (st, ft) =>
                       elift2 (fun sofarT eT =>
                                 let et := exprct_type_annot eT in
-                                let sofart := ergoc_type_join et (snd sofarT) in
+                                let sofart := qcert_type_join et (snd sofarT) in
                                 ((CaseLetOption (prov,sofart) name None,eT)::fst sofarT, sofart))
                              sofarT
-                             (ergoc_typecheck_expr nsctxt (type_context_update_local_env ctxt name st) res)
+                             (ergoc_expr_typecheck nsctxt (type_context_update_local_env ctxt name st) res)
                     end
                   | (CaseLetOption prov name (Some b), res) =>
                     match unteither t0 with
@@ -281,10 +281,10 @@ Section ErgoCTypecheck.
                     | Some (st, ft) =>
                       elift2 (fun sofarT eT =>
                                 let et := exprct_type_annot eT in
-                                let sofart := ergoc_type_join et (snd sofarT) in
+                                let sofart := qcert_type_join et (snd sofarT) in
                                 ((CaseLetOption (prov,sofart) name (Some b), eT)::fst sofarT, sofart))
                              sofarT
-                             (ergoc_typecheck_expr
+                             (ergoc_expr_typecheck
                                 nsctxt (type_context_update_local_env
                                           ctxt
                                           name
@@ -296,12 +296,12 @@ Section ErgoCTypecheck.
                               let sofart := snd sofarT in
                               ((CaseWildcard (prov,sofart) (Some b), eT)::fst sofarT, sofart))
                            sofarT
-                           (ergoc_typecheck_expr nsctxt ctxt res)
+                           (ergoc_expr_typecheck nsctxt ctxt res)
                   end)
                (esuccess (nil, dt) nil)
                pes))
-        (ergoc_typecheck_expr nsctxt ctxt term)
-        (ergoc_typecheck_expr nsctxt ctxt default)
+        (ergoc_expr_typecheck nsctxt ctxt term)
+        (ergoc_expr_typecheck nsctxt ctxt default)
     (* EXPECTS: each foreach has only one dimension and no where *)
     | EForeach prov ((name,arr)::nil) None fn =>
       eolift
@@ -311,18 +311,18 @@ Section ErgoCTypecheck.
              (fun typ =>
                 (elift
                    (fun eT => EForeach (prov, tcoll (exprct_type_annot eT)) ((name,arrT')::nil) None eT)
-                   (ergoc_typecheck_expr nsctxt (type_context_update_local_env ctxt name typ) fn)))
+                   (ergoc_expr_typecheck nsctxt (type_context_update_local_env ctxt name typ) fn)))
              (eresult_of_option
                 (untcoll arr')
                 (ETypeError
                    prov
-                   ("foreach expects an array to iterate over, but was given something of type `" ++ (ergoc_type_to_string nsctxt arr') ++ "'.")) nil))
-        (ergoc_typecheck_expr nsctxt ctxt arr)
+                   ("foreach expects an array to iterate over, but was given something of type `" ++ (qcert_type_to_string nsctxt arr') ++ "'.")) nil))
+        (ergoc_expr_typecheck nsctxt ctxt arr)
     | EForeach prov _ _ _ =>
       complex_foreach_in_calculus_error prov
     end.
 
-  Definition ergoc_typecheck_function
+  Definition ergoc_function_typecheck
              (nsctxt: namespace_ctxt)
              (name:string)
              (dctxt : type_context)
@@ -335,7 +335,7 @@ Section ErgoCTypecheck.
                         dctxt) nil
     | Some body =>
       let tsig :=
-          map (fun x => (fst x, ergo_type_to_ergoc_type (snd x)))
+          map (fun x => (fst x, ergo_type_to_qcert_type (snd x)))
               func.(functionc_sig).(sigc_params) in
       eolift
         (fun outT =>
@@ -348,7 +348,7 @@ Section ErgoCTypecheck.
                                  (Some outT),
                                dctxt) nil
            | Some eoutt' =>
-             let expectedt := ergo_type_to_ergoc_type eoutt' in
+             let expectedt := ergo_type_to_qcert_type eoutt' in
              if subtype_dec outt expectedt
              then esuccess (mkFuncCT
                               func.(functionc_annot)
@@ -366,17 +366,17 @@ Section ErgoCTypecheck.
                  efailure (ETypeError body_prov (ergo_format_function_return_error nsctxt name outt expectedt))
                end
            end)
-        (ergoc_typecheck_expr nsctxt (type_context_set_local_env dctxt tsig) body)
+        (ergoc_expr_typecheck nsctxt (type_context_set_local_env dctxt tsig) body)
     end.
 
-  Definition ergoc_typecheck_clause
+  Definition ergoc_clause_typecheck
              (nsctxt: namespace_ctxt)
              (dctxt : type_context)
              (cl : string * ergoc_function) : eresult ((string * ergoct_function) * type_context) :=
     let (name,body) := cl in
-    elift (fun fT => ((name,fst fT), snd fT)) (ergoc_typecheck_function nsctxt name dctxt body).
+    elift (fun fT => ((name,fst fT), snd fT)) (ergoc_function_typecheck nsctxt name dctxt body).
 
-  Definition ergoc_typecheck_contract
+  Definition ergoc_contract_typecheck
              (nsctxt: namespace_ctxt)
              (dctxt : type_context)
              (coname: absolute_name)
@@ -387,21 +387,21 @@ Section ErgoCTypecheck.
                 (fst cT),
               snd cT))
           (elift_context_fold_left
-             (ergoc_typecheck_clause nsctxt)
+             (ergoc_clause_typecheck nsctxt)
              c.(contractc_clauses)
              dctxt).
 
-  Definition ergoc_typecheck_decl
+  Definition ergoc_decl_typecheck
              (nsctxt: namespace_ctxt)
              (dctxt : type_context)
              (decl : ergoc_declaration)
     : eresult (ergoct_declaration * type_context) :=
     match decl with
     | DCExpr prov expr =>
-      let exprT := ergoc_typecheck_expr nsctxt dctxt expr in
+      let exprT := ergoc_expr_typecheck nsctxt dctxt expr in
       elift (fun xT => (DCTExpr (prov, exprct_type_annot xT) xT, dctxt)) exprT
     | DCConstant prov name None expr =>
-      let exprT := ergoc_typecheck_expr nsctxt dctxt expr in
+      let exprT := ergoc_expr_typecheck nsctxt dctxt expr in
       elift (fun xT => (DCTConstant (prov,exprct_type_annot xT) name None xT,
                         type_context_update_global_env dctxt name (exprct_type_annot xT)))
             exprT
@@ -410,18 +410,18 @@ Section ErgoCTypecheck.
           fun t' vt =>
             ETypeError prov
                        ("The type annotation `"
-                          ++ (ergoc_type_to_string nsctxt t')
+                          ++ (qcert_type_to_string nsctxt t')
                           ++ "' for the constant `"
                           ++ name
                           ++ "' does not match its actual type `"
-                          ++ (ergoc_type_to_string nsctxt vt)
+                          ++ (qcert_type_to_string nsctxt vt)
                           ++ "'.")
       in
-      let exprT := ergoc_typecheck_expr nsctxt dctxt expr in
+      let exprT := ergoc_expr_typecheck nsctxt dctxt expr in
       eolift
         (fun vT =>
            let vt := exprct_type_annot vT in
-           let t' := (ergo_type_to_ergoc_type t) in
+           let t' := (ergo_type_to_qcert_type t) in
            if subtype_dec vt t' then
              let ctxt' := type_context_update_global_env dctxt name t' in
              esuccess (DCTConstant (prov,t') name (Some t) vT, ctxt') nil
@@ -430,13 +430,13 @@ Section ErgoCTypecheck.
         exprT
     | DCFunc prov name func =>
       elift (fun fc => (DCTFunc prov name (fst fc),snd fc))
-            (ergoc_typecheck_function nsctxt name dctxt func)
+            (ergoc_function_typecheck nsctxt name dctxt func)
     | DCContract prov name contr =>
       elift (fun fc => (DCTContract prov name (fst fc),snd fc))
-            (ergoc_typecheck_contract nsctxt dctxt name contr)
+            (ergoc_contract_typecheck nsctxt dctxt name contr)
     end.
 
-  Definition ergoc_typecheck_module
+  Definition ergoc_module_typecheck
              (nsctxt: namespace_ctxt)
              (dctxt : type_context)
              (mod : ergoc_module)
@@ -447,7 +447,7 @@ Section ErgoCTypecheck.
                       (fst x),
                      snd x))
           (elift_context_fold_left
-             (ergoc_typecheck_decl nsctxt)
+             (ergoc_decl_typecheck nsctxt)
              mod.(modulec_declarations)
              dctxt).
   
