compiler/core/Types/QcertTypeUtil.v
@@ -12,7 +12,7 @@
  * limitations under the License.
  *)
 
-(* Support for ErgoType models *)
+(* Support for Qcert types *)
 
 Require Import String.
 Require Import List.
@@ -25,58 +25,58 @@ Require Import ErgoSpec.Common.Result.
 Require Import ErgoSpec.Common.Ast.
 Require Import ErgoSpec.Common.PrintTypedData.
 
-Section ErgoCTypeUtil.
+Section QcertTypeUtil.
   Context {m : brand_model}.
 
   Import QcertType.
 
-  Definition ergoc_type_join_safe prov (t1 t2:ergoc_type) : eresult ergoc_type :=
-    let jt := ergoc_type_join t1 t2 in
-    if ergoc_type_subtype_dec ttop jt
+  Definition qcert_type_join_safe prov (t1 t2:qcert_type) : eresult qcert_type :=
+    let jt := qcert_type_join t1 t2 in
+    if qcert_type_subtype_dec ttop jt
     then efailure (ETypeError prov ("Join between types is TOP.")%string)
     else esuccess jt nil.
 
-  Definition ergoc_type_meet_safe prov (t1 t2:ergoc_type) : eresult ergoc_type :=
-    let jt := ergoc_type_meet t1 t2 in
-    if ergoc_type_subtype_dec jt tbottom
+  Definition qcert_type_meet_safe prov (t1 t2:qcert_type) : eresult qcert_type :=
+    let jt := qcert_type_meet t1 t2 in
+    if qcert_type_subtype_dec jt tbottom
     then efailure (ETypeError prov ("Meet between types is BOTTOM.")%string)
     else esuccess jt nil.
 
-  Program Definition empty_rec_type : ergoc_type := Rec Closed nil _.
+  Program Definition empty_rec_type : qcert_type := Rec Closed nil _.
 
-  Definition ergo_format_unop_error nsctxt (op : unary_op) (arg : ergoc_type) : string :=
+  Definition ergo_format_unop_error nsctxt (op : unary_op) (arg : qcert_type) : string :=
     let fmt_easy :=
         fun name expected actual =>
           ("Operator `" ++ name ++ "' expected an operand of type `" ++
-                        (ergoc_type_to_string nsctxt expected) ++
+                        (qcert_type_to_string nsctxt expected) ++
                         "' but received an operand of type `" ++
-                        (ergoc_type_to_string nsctxt actual) ++ "'.")%string
+                        (qcert_type_to_string nsctxt actual) ++ "'.")%string
     in
     match op with
     | OpNeg => fmt_easy "!"%string tbool arg
     | OpFloatUnary FloatNeg => fmt_easy "-"%string tfloat arg
-    | OpDot name => "The field `" ++ name ++ "' does not exist in type `" ++ (ergoc_type_to_string nsctxt arg) ++ "'"
+    | OpDot name => "The field `" ++ name ++ "' does not exist in type `" ++ (qcert_type_to_string nsctxt arg) ++ "'"
     | OpIdentity | OpRec _ | OpBag
     | OpLeft | OpRight | OpBrand _ | OpUnbrand | OpCast _ =>
-      "This operator received an unexpected argument of type `" ++ (ergoc_type_to_string nsctxt arg) ++ "'"
+      "This operator received an unexpected argument of type `" ++ (qcert_type_to_string nsctxt arg) ++ "'"
     | OpRecRemove _ | OpRecProject _
     | OpSingleton | OpFlatten | OpDistinct | OpOrderBy _
     | OpCount | OpToString | OpToText | OpLength | OpSubstring _ _ | OpLike _
     | OpNatUnary _ | OpNatSum | OpNatMin | OpNatMax | OpNatMean | OpFloatOfNat
     | OpFloatUnary _ | OpFloatTruncate | OpFloatSum | OpFloatMean | OpFloatBagMin | OpFloatBagMax
     | OpForeignUnary _ =>
-      "This function received an unexpected argument of type `" ++ (ergoc_type_to_string nsctxt arg) ++ "'"
+      "This function received an unexpected argument of type `" ++ (qcert_type_to_string nsctxt arg) ++ "'"
     end.
 
-  Definition ergo_format_binop_error nsctxt (op : binary_op) (arg1 : ergoc_type) (arg2 : ergoc_type) : string :=
+  Definition ergo_format_binop_error nsctxt (op : binary_op) (arg1 : qcert_type) (arg2 : qcert_type) : string :=
     let fmt_easy :=
         fun name e1 e2 =>
           ("Operator `" ++ name ++ "' expected operands of type `" ++
-                        (ergoc_type_to_string nsctxt e1) ++ "' and `" ++
-                        (ergoc_type_to_string nsctxt e2) ++
+                        (qcert_type_to_string nsctxt e1) ++ "' and `" ++
+                        (qcert_type_to_string nsctxt e2) ++
                         "' but received operands of type `" ++
-                        (ergoc_type_to_string nsctxt arg1) ++ "' and `" ++
-                        (ergoc_type_to_string nsctxt arg2) ++ "'.")%string
+                        (qcert_type_to_string nsctxt arg1) ++ "' and `" ++
+                        (qcert_type_to_string nsctxt arg2) ++ "'.")%string
     in
     match op with
     | OpAnd => fmt_easy "and"%string tbool tbool
@@ -99,23 +99,23 @@ Section ErgoCTypeUtil.
     | OpFloatCompare FloatGe => fmt_easy ">="%string tfloat tfloat
     | OpRecConcat | OpRecMerge
     | OpEqual | OpStringConcat | OpStringJoin
-      => "This operator received unexpected arguments of type `" ++ (ergoc_type_to_string nsctxt arg1) ++ "' " ++ " and `" ++ (ergoc_type_to_string nsctxt arg2) ++ "'."
+      => "This operator received unexpected arguments of type `" ++ (qcert_type_to_string nsctxt arg1) ++ "' " ++ " and `" ++ (qcert_type_to_string nsctxt arg2) ++ "'."
     | OpBagUnion | OpBagDiff | OpBagMin | OpBagMax | OpBagNth | OpContains
     | OpFloatBinary FloatMin | OpFloatBinary FloatMax
     | OpForeignBinary _
-      => "This function received unexpected arguments of type `" ++ (ergoc_type_to_string nsctxt arg1) ++ "' " ++ " and `" ++ (ergoc_type_to_string nsctxt arg2) ++ "'."
+      => "This function received unexpected arguments of type `" ++ (qcert_type_to_string nsctxt arg1) ++ "' " ++ " and `" ++ (qcert_type_to_string nsctxt arg2) ++ "'."
     end.
 
   Definition ergo_format_unary_operator_dispatch_error nsctxt (op : ergo_unary_operator)
-     (arg : ergoc_type) : string :=
-    "This operator received an unexpected argument of type `" ++ (ergoc_type_to_string nsctxt arg) ++ "'.".
+     (arg : qcert_type) : string :=
+    "This operator received an unexpected argument of type `" ++ (qcert_type_to_string nsctxt arg) ++ "'.".
 
   Definition ergo_format_binary_operator_dispatch_error nsctxt (op : ergo_binary_operator)
-     (arg1 : ergoc_type) (arg2 : ergoc_type) : string :=
-    "This operator received unexpected arguments of type `" ++ (ergoc_type_to_string nsctxt arg1) ++ "' " ++ " and `" ++ (ergoc_type_to_string nsctxt arg2) ++ "'.".
+     (arg1 : qcert_type) (arg2 : qcert_type) : string :=
+    "This operator received unexpected arguments of type `" ++ (qcert_type_to_string nsctxt arg1) ++ "' " ++ " and `" ++ (qcert_type_to_string nsctxt arg2) ++ "'.".
 
-  Definition ergo_format_new_error nsctxt (name:string) (actual:ergoc_type) : string :=
-    let concept_name := ergoc_type_to_string nsctxt (Brand (name::nil)) in
+  Definition ergo_format_new_error nsctxt (name:string) (actual:qcert_type) : string :=
+    let concept_name := qcert_type_to_string nsctxt (Brand (name::nil)) in
     (* First check if all the fields are present and no extra field is present *)
     match diff_record_types (name::nil) actual with
     | None => "Concept name " ++ name ++ " does not match data"
@@ -125,8 +125,8 @@ Section ErgoCTypeUtil.
       | nil => "Concept " ++ name ++ " doesn't match data (one field is not a subtype)"
       | (expected_name, expected_type, actual_type) :: _ =>
         "Field `" ++ expected_name
-                  ++ "' has type `" ++ (ergoc_type_to_string nsctxt actual_type)
-                  ++ "' but should have type `" ++ (ergoc_type_to_string nsctxt expected_type) ++ "'"
+                  ++ "' has type `" ++ (qcert_type_to_string nsctxt actual_type)
+                  ++ "' but should have type `" ++ (qcert_type_to_string nsctxt expected_type) ++ "'"
       end
     | Some (nil, actual_name::nil) =>
       "Unknown field `" ++ actual_name ++ "' in type `" ++ concept_name ++ "'"
@@ -141,9 +141,9 @@ Section ErgoCTypeUtil.
   Definition ergo_format_clause_return_fallback_error
              nsctxt
              (name:string)
-             (actual expected:ergoc_type) : string :=
-    let actual_s := ergoc_type_to_string nsctxt actual in
-    let expected_s := ergoc_type_to_string nsctxt expected in
+             (actual expected:qcert_type) : string :=
+    let actual_s := qcert_type_to_string nsctxt actual in
+    let expected_s := qcert_type_to_string nsctxt expected in
     "Clause " ++ name ++ " should return `" ++ expected_s
               ++ "' but actually returns `" ++ actual_s ++ "'".
 
@@ -151,27 +151,27 @@ Section ErgoCTypeUtil.
              nsctxt
              (name:string)
              (component1 component2:string)
-             (actual expected:ergoc_type) : string :=
-    let actual_s := ergoc_type_to_string nsctxt actual in
-    let expected_s := ergoc_type_to_string nsctxt expected in
+             (actual expected:qcert_type) : string :=
+    let actual_s := qcert_type_to_string nsctxt actual in
+    let expected_s := qcert_type_to_string nsctxt expected in
     "Clause " ++ name ++ " should " ++ component1 ++ " `" ++ expected_s
               ++ "' but actually " ++ component2 ++ " `" ++ actual_s ++ "'".
 
   Definition ergo_format_clause_return_normal_error
              nsctxt
              (name:string)
-             (actual expected:ergoc_type)
-             (actual_quad expected_quad:ergoc_type * ergoc_type * ergoc_type * ergoc_type)
+             (actual expected:qcert_type)
+             (actual_quad expected_quad:qcert_type * qcert_type * qcert_type * qcert_type)
     : string :=
     let '(actual_resp, actual_emit, actual_state, actual_error) := actual_quad in
     let '(expected_resp, expected_emit, expected_state, expected_error) := expected_quad in
-    if ergoc_type_subtype_dec actual_resp expected_resp
+    if qcert_type_subtype_dec actual_resp expected_resp
     then
-      if ergoc_type_subtype_dec actual_emit expected_emit
+      if qcert_type_subtype_dec actual_emit expected_emit
       then
-        if ergoc_type_subtype_dec actual_state expected_state
+        if qcert_type_subtype_dec actual_state expected_state
         then
-          if ergoc_type_subtype_dec actual_error expected_error
+          if qcert_type_subtype_dec actual_error expected_error
           then
             ergo_format_clause_return_fallback_error nsctxt name actual expected
           else
@@ -187,7 +187,7 @@ Section ErgoCTypeUtil.
       ergo_format_clause_return_component_error
         nsctxt name "respond" "responds" actual_resp expected_resp.
 
-  Definition ergo_format_clause_return_error nsctxt (name:string) (actual expected:ergoc_type) : string :=
+  Definition ergo_format_clause_return_error nsctxt (name:string) (actual expected:qcert_type) : string :=
     let actual_quad := unpack_output_type nsctxt actual nil in
     let expected_quad := unpack_output_type nsctxt expected nil in
     let normal_error := ergo_format_clause_return_normal_error nsctxt name actual expected in
@@ -198,21 +198,21 @@ Section ErgoCTypeUtil.
       actual_quad
       expected_quad.
   
-  Definition ergo_format_function_return_error nsctxt (name:string) (actual expected:ergoc_type) : string :=
-    let actual_s := ergoc_type_to_string nsctxt actual in
-    let expected_s := ergoc_type_to_string nsctxt expected in
+  Definition ergo_format_function_return_error nsctxt (name:string) (actual expected:qcert_type) : string :=
+    let actual_s := qcert_type_to_string nsctxt actual in
+    let expected_s := qcert_type_to_string nsctxt expected in
     "Function " ++ name ++ " should return `" ++ expected_s ++ "' but actually returns `" ++ actual_s ++ "'".
 
-  Definition make_unary_operator_criteria op nsctxt prov t : eresult ergoc_type :=
-    match ergoc_type_infer_unary_op op t with
+  Definition make_unary_operator_criteria op nsctxt prov t : eresult qcert_type :=
+    match qcert_type_infer_unary_op op t with
     | Some (r, _) => esuccess r nil
     | None => efailure (ETypeError prov (ergo_format_unop_error nsctxt op t))
     end.
 
-  Definition make_binary_operator_criteria op nsctxt prov t1 t2 : eresult ergoc_type :=
-    match ergoc_type_infer_binary_op op t1 t2 with
+  Definition make_binary_operator_criteria op nsctxt prov t1 t2 : eresult qcert_type :=
+    match qcert_type_infer_binary_op op t1 t2 with
     | Some (r, _, _) => esuccess r nil
     | None => efailure (ETypeError prov (ergo_format_binop_error nsctxt op t1 t2))
     end.
 
-End ErgoCTypeUtil.
+End QcertTypeUtil.
